rt refine RISCV: update for MCS till end of KHeap_R.thy
Signed-off-by: Michael McInerney <m.mcinerney@unsw.edu.au>

proof/refine/RISCV64/Invariants_H.thy
@@ -7,7 +7,9 @@
 theory Invariants_H
 imports
   LevityCatch
-  "AInvs.ArchDetSchedSchedule_AI"
+  "AInvs.AInvs"
+  "Lib.AddUpdSimps"
+  ArchMove_R
 begin
 
 (* global data and code of the kernel, not covered by any cap *)
@@ -37,6 +39,20 @@ end
 
 end
 
+section "Relationship of Executable Spec to Kernel Configuration"
+
+text \<open>
+  Some values are set per kernel configuration (e.g. number of domains), but other related
+  values (e.g. maximum domain) are derived from storage constraints (e.g. bytes used).
+  To relate the two, we must look at the values of kernel configuration constants.
+  To allow the proofs to work for all permitted values of these constants, their definitions
+  should only be unfolded in this section, and the derived properties kept to a minimum.\<close>
+
+lemma le_maxDomain_eq_less_numDomains:
+  shows "x \<le> unat maxDomain \<longleftrightarrow> x < Kernel_Config.numDomains"
+        "y \<le> maxDomain \<longleftrightarrow> unat y < Kernel_Config.numDomains"
+  by (auto simp: Kernel_Config.numDomains_def maxDomain_def word_le_nat_alt)
+
 \<comment> \<open>---------------------------------------------------------------------------\<close>
 
 section "Invariants on Executable Spec"
@@ -53,7 +69,18 @@ definition pspace_no_overlap' :: "obj_ref \<Rightarrow> nat \<Rightarrow> kernel
 
 definition ko_wp_at' :: "(kernel_object \<Rightarrow> bool) \<Rightarrow> obj_ref \<Rightarrow> kernel_state \<Rightarrow> bool" where
   "ko_wp_at' P p s \<equiv> \<exists>ko. ksPSpace s p = Some ko \<and> is_aligned p (objBitsKO ko) \<and> P ko \<and>
-                           ps_clear p (objBitsKO ko) s"
+                           ps_clear p (objBitsKO ko) s \<and> objBitsKO ko < word_bits"
+
+lemma valid_sz_simps:
+  "objBitsKO ko < word_bits =
+    (case ko of
+      (KOSchedContext sc) \<Rightarrow> scBitsFromRefillLength sc < word_bits
+      | _ \<Rightarrow>    True)"
+  by (cases ko;
+      clarsimp simp: objBits_def objBitsKO_def word_size_def archObjSize_def pageBits_def word_bits_def
+                     tcbBlockSizeBits_def epSizeBits_def ntfnSizeBits_def cteSizeBits_def word_size
+                     pteBits_def wordSizeCase_def wordBits_def replySizeBits_def
+              split: arch_kernel_object.splits)
 
 definition obj_at' :: "('a::pspace_storable \<Rightarrow> bool) \<Rightarrow> machine_word \<Rightarrow> kernel_state \<Rightarrow> bool" where
   obj_at'_real_def:
@@ -74,6 +101,12 @@ abbreviation tcb_at' :: "obj_ref \<Rightarrow> kernel_state \<Rightarrow> bool" 
 abbreviation real_cte_at' :: "obj_ref \<Rightarrow> kernel_state \<Rightarrow> bool" where
   "real_cte_at' \<equiv> obj_at' ((\<lambda>x. True) :: cte \<Rightarrow> bool)"
 
+abbreviation sc_at' :: "obj_ref \<Rightarrow> kernel_state \<Rightarrow> bool" where
+  "sc_at' \<equiv> obj_at' (\<lambda>_ :: sched_context. True)"
+
+abbreviation reply_at' :: "obj_ref \<Rightarrow> kernel_state \<Rightarrow> bool" where
+  "reply_at' \<equiv> obj_at' (\<lambda>_ :: reply. True)"
+
 abbreviation ko_at' :: "'a::pspace_storable \<Rightarrow> obj_ref \<Rightarrow> kernel_state \<Rightarrow> bool" where
   "ko_at' v \<equiv> obj_at' (\<lambda>k. k = v)"
 
@@ -84,33 +117,33 @@ end
 
 record itcb' =
   itcbState             :: thread_state
-  itcbFaultHandler      :: cptr
   itcbIPCBuffer         :: vptr
   itcbBoundNotification :: "machine_word option"
   itcbPriority          :: priority
   itcbFault             :: "fault option"
-  itcbTimeSlice         :: nat
   itcbMCP               :: priority
+  itcbSchedContext      :: "obj_ref option"
+  itcbYieldTo           :: "obj_ref option"
 
 definition tcb_to_itcb' :: "tcb \<Rightarrow> itcb'" where
   "tcb_to_itcb' tcb \<equiv> \<lparr> itcbState             = tcbState tcb,
-                        itcbFaultHandler      = tcbFaultHandler tcb,
                         itcbIPCBuffer         = tcbIPCBuffer tcb,
                         itcbBoundNotification = tcbBoundNotification tcb,
                         itcbPriority          = tcbPriority tcb,
                         itcbFault             = tcbFault tcb,
-                        itcbTimeSlice         = tcbTimeSlice tcb,
-                        itcbMCP               = tcbMCP tcb\<rparr>"
+                        itcbMCP               = tcbMCP tcb,
+                        itcbSchedContext      = tcbSchedContext tcb,
+                        itcbYieldTo           = tcbYieldTo tcb\<rparr>"
 
 lemma itcb_simps[simp]:
   "itcbState (tcb_to_itcb' tcb) = tcbState tcb"
-  "itcbFaultHandler (tcb_to_itcb' tcb) = tcbFaultHandler tcb"
   "itcbIPCBuffer (tcb_to_itcb' tcb) = tcbIPCBuffer tcb"
   "itcbBoundNotification (tcb_to_itcb' tcb) = tcbBoundNotification tcb"
   "itcbPriority (tcb_to_itcb' tcb) = tcbPriority tcb"
   "itcbFault (tcb_to_itcb' tcb) = tcbFault tcb"
-  "itcbTimeSlice (tcb_to_itcb' tcb) = tcbTimeSlice tcb"
   "itcbMCP (tcb_to_itcb' tcb) = tcbMCP tcb"
+  "itcbSchedContext (tcb_to_itcb' tcb) = tcbSchedContext tcb"
+  "itcbYieldTo (tcb_to_itcb' tcb) = tcbYieldTo tcb"
   by (auto simp: tcb_to_itcb'_def)
 
 definition pred_tcb_at' :: "(itcb' \<Rightarrow> 'a) \<Rightarrow> ('a \<Rightarrow> bool) \<Rightarrow> machine_word \<Rightarrow> kernel_state \<Rightarrow> bool"
@@ -130,6 +163,9 @@ lemma st_tcb_at'_def:
   "st_tcb_at' test \<equiv> obj_at' (test \<circ> tcbState)"
   by (simp add: pred_tcb_at'_def o_def)
 
+definition active_sc_at' :: "obj_ref \<Rightarrow> kernel_state \<Rightarrow> bool" where
+  "active_sc_at' \<equiv> obj_at' (\<lambda>ko :: sched_context. 0 < scRefillMax ko)"
+
 text \<open> cte with property at \<close>
 definition cte_wp_at' :: "(cte \<Rightarrow> bool) \<Rightarrow> obj_ref \<Rightarrow> kernel_state \<Rightarrow> bool" where
   "cte_wp_at' P p s \<equiv> \<exists>cte::cte. fst (getObject p s) = {(cte,s)} \<and> P cte"
@@ -137,67 +173,217 @@ definition cte_wp_at' :: "(cte \<Rightarrow> bool) \<Rightarrow> obj_ref \<Right
 abbreviation cte_at' :: "obj_ref \<Rightarrow> kernel_state \<Rightarrow> bool" where
   "cte_at' \<equiv> cte_wp_at' \<top>"
 
+text \<open>replyNext aliases\<close>
+
+abbreviation replySC :: "reply \<Rightarrow> obj_ref option" where
+  "replySC \<equiv> \<lambda>r. getHeadScPtr (replyNext r)"
+
+abbreviation replyNext_of :: "reply \<Rightarrow> obj_ref option" where
+  "replyNext_of \<equiv> \<lambda>r. getReplyNextPtr (replyNext r)"
+
+lemmas getReplyNextPr_simps[simp] = getReplyNextPtr_def[split_simps option.split reply_next.split]
+
+lemmas getHeadScPtr_simps[simp] = getHeadScPtr_def[split_simps option.split reply_next.split]
+
+lemma getReplyNextPtr_Some_iff[iff]:
+  "(getReplyNextPtr x) = (Some rn) \<longleftrightarrow> x = Some (Next rn)"
+  by (cases x; clarsimp simp: getReplyNextPtr_def split: reply_next.split)
+
+lemma getHeadScPtr_Some_iff[iff]:
+  "(getHeadScPtr x) = (Some rn) \<longleftrightarrow> x = Some (Head rn)"
+  by (cases x; clarsimp simp: getHeadScPtr_def split: reply_next.split)
+
+lemma getReplyNextPtr_None_iff:
+  "(getReplyNextPtr x) = None \<longleftrightarrow> (\<forall>rn. x \<noteq> Some (Next rn))"
+  by (cases x; clarsimp simp: getReplyNextPtr_def split: reply_next.split)
+
+lemma getHeadScPtr_None_iff:
+  "(getHeadScPtr x) = None \<longleftrightarrow> (\<forall>rn. x \<noteq> Some (Head rn))"
+  by (cases x; clarsimp simp: getHeadScPtr_def split: reply_next.split)
+
+lemma replyNext_None_iff:
+  "replyNext r = None \<longleftrightarrow> replyNext_of r = None \<and> replySC r = None"
+  apply (cases "replyNext r"; clarsimp)
+  apply (case_tac a; clarsimp)
+  done
+
+lemma getReplyNextPtr_Head_None[simp]:
+  "getReplyNextPtr (Some (Head rn)) = None" by (simp add: getReplyNextPtr_def)
+
+lemma getHeadScPtr_Next_None[simp]:
+  "getHeadScPtr (Some (Next sc)) = None" by (simp add: getHeadScPtr_def)
+
+text \<open>Heap projections:\<close>
+abbreviation reply_of' :: "kernel_object \<Rightarrow> reply option" where
+  "reply_of' \<equiv> projectKO_opt"
+
+abbreviation replies_of' :: "kernel_state \<Rightarrow> obj_ref \<Rightarrow> reply option" where
+  "replies_of' s \<equiv> ksPSpace s |> reply_of'"
+
+abbreviation replyNexts_of :: "kernel_state \<Rightarrow> obj_ref \<Rightarrow> obj_ref option" where
+  "replyNexts_of s \<equiv> replies_of' s |> replyNext_of"
+
+abbreviation replyPrevs_of :: "kernel_state \<Rightarrow> obj_ref \<Rightarrow> obj_ref option" where
+  "replyPrevs_of s \<equiv> replies_of' s |> replyPrev"
+
+abbreviation replyTCBs_of :: "kernel_state \<Rightarrow> obj_ref \<Rightarrow> obj_ref option" where
+  "replyTCBs_of s \<equiv> replies_of' s |> replyTCB"
+
+abbreviation replySCs_of :: "kernel_state \<Rightarrow> obj_ref \<Rightarrow> obj_ref option" where
+  "replySCs_of s \<equiv> replies_of' s |> replySC"
+
+abbreviation sc_of' :: "kernel_object \<Rightarrow> sched_context option" where
+  "sc_of' \<equiv> projectKO_opt"
+
+abbreviation scs_of' :: "kernel_state \<Rightarrow> obj_ref \<Rightarrow> sched_context option" where
+  "scs_of' s \<equiv> ksPSpace s |> sc_of'"
+
+abbreviation scReplies_of :: "kernel_state \<Rightarrow> obj_ref \<Rightarrow> obj_ref option" where
+  "scReplies_of s \<equiv> scs_of' s |> scReply"
+
+abbreviation tcb_of' :: "kernel_object \<Rightarrow> tcb option" where
+  "tcb_of' \<equiv> projectKO_opt"
+
+abbreviation tcbs_of' :: "kernel_state \<Rightarrow> obj_ref \<Rightarrow> tcb option" where
+  "tcbs_of' s \<equiv> ksPSpace s |> tcb_of'"
+
+abbreviation tcbSCs_of :: "kernel_state \<Rightarrow> obj_ref \<Rightarrow> obj_ref option" where
+  "tcbSCs_of s \<equiv> tcbs_of' s |> tcbSchedContext"
+
+abbreviation scTCBs_of :: "kernel_state \<Rightarrow> obj_ref \<Rightarrow> obj_ref option" where
+  "scTCBs_of s \<equiv> scs_of' s |> scTCB"
+
+abbreviation sym_heap_tcbSCs where
+  "sym_heap_tcbSCs s \<equiv> sym_heap (tcbSCs_of s) (scTCBs_of s)"
+
+abbreviation sym_heap_scReplies where
+  "sym_heap_scReplies s \<equiv> sym_heap (scReplies_of s) (replySCs_of s)"
+
 definition tcb_cte_cases :: "machine_word \<rightharpoonup> ((tcb \<Rightarrow> cte) \<times> ((cte \<Rightarrow> cte) \<Rightarrow> tcb \<Rightarrow> tcb))" where
  "tcb_cte_cases \<equiv> [ 0 << cteSizeBits \<mapsto> (tcbCTable, tcbCTable_update),
                     1 << cteSizeBits \<mapsto> (tcbVTable, tcbVTable_update),
-                    2 << cteSizeBits \<mapsto> (tcbReply, tcbReply_update),
-                    3 << cteSizeBits \<mapsto> (tcbCaller, tcbCaller_update),
-                    4 << cteSizeBits \<mapsto> (tcbIPCBufferFrame, tcbIPCBufferFrame_update) ]"
+                    2 << cteSizeBits \<mapsto> (tcbIPCBufferFrame, tcbIPCBufferFrame_update),
+                    3 << cteSizeBits \<mapsto> (tcbFaultHandler, tcbFaultHandler_update),
+                    4 << cteSizeBits \<mapsto> (tcbTimeoutHandler, tcbTimeoutHandler_update) ]"
 
 definition max_ipc_words :: machine_word where
   "max_ipc_words \<equiv> capTransferDataSize + msgMaxLength + msgMaxExtraCaps + 2"
 
-definition tcb_st_refs_of' :: "thread_state \<Rightarrow> (obj_ref \<times> reftype) set" where
-  "tcb_st_refs_of' st \<equiv> case st of
-     (BlockedOnReceive x _)     => {(x, TCBBlockedRecv)}
-   | (BlockedOnSend x _ _ _ _)  => {(x, TCBBlockedSend)}
-   | (BlockedOnNotification x)  => {(x, TCBSignal)}
-   | _                          => {}"
+type_synonym ref_set = "(obj_ref \<times> reftype) set"
+
+definition tcb_st_refs_of' :: "thread_state \<Rightarrow> ref_set" where
+  "tcb_st_refs_of' z \<equiv> case z of
+    BlockedOnReply r          \<Rightarrow> if bound r then {(the r, TCBReply)} else {}
+  | BlockedOnReceive x _ r    \<Rightarrow> if bound r then {(x, TCBBlockedRecv), (the r, TCBReply)}
+                                    else {(x, TCBBlockedRecv)}
+  | BlockedOnSend x _ _ _ _   \<Rightarrow> {(x, TCBBlockedSend)}
+  | BlockedOnNotification x   \<Rightarrow> {(x, TCBSignal)}
+  | _                         \<Rightarrow> {}"
+
+definition tcb_bound_refs' :: "obj_ref option \<Rightarrow> obj_ref option \<Rightarrow> obj_ref option \<Rightarrow> ref_set" where
+  "tcb_bound_refs' ntfn sc yt \<equiv> get_refs TCBBound ntfn
+                                  \<union> get_refs TCBSchedContext sc
+                                  \<union> get_refs TCBYieldTo yt"
+
+definition refs_of_tcb' :: "tcb \<Rightarrow> ref_set" where
+  "refs_of_tcb' tcb \<equiv>
+     tcb_st_refs_of' (tcbState tcb)
+       \<union> tcb_bound_refs' (tcbBoundNotification tcb) (tcbSchedContext tcb) (tcbYieldTo tcb)"
 
 definition ep_q_refs_of' :: "endpoint \<Rightarrow> (obj_ref \<times> reftype) set" where
   "ep_q_refs_of' ep \<equiv> case ep of
      IdleEP     => {}
-   | (RecvEP q) => set q \<times> {EPRecv}
-   | (SendEP q) => set q \<times> {EPSend}"
+   | RecvEP q => set q \<times> {EPRecv}
+   | SendEP q => set q \<times> {EPSend}"
 
 definition ntfn_q_refs_of' :: "Structures_H.ntfn \<Rightarrow> (obj_ref \<times> reftype) set" where
   "ntfn_q_refs_of' ntfn \<equiv> case ntfn of
      IdleNtfn        => {}
-   | (WaitingNtfn q) => set q \<times> {NTFNSignal}
-   | (ActiveNtfn b)  => {}"
+   | WaitingNtfn q   => set q \<times> {NTFNSignal}
+   | ActiveNtfn b    => {}"
 
 definition ntfn_bound_refs' :: "obj_ref option \<Rightarrow> (obj_ref \<times> reftype) set" where
   "ntfn_bound_refs' t \<equiv> set_option t \<times> {NTFNBound}"
 
-definition tcb_bound_refs' :: "obj_ref option \<Rightarrow> (obj_ref \<times> reftype) set" where
-  "tcb_bound_refs' a \<equiv> set_option a \<times> {TCBBound}"
+definition refs_of_ntfn' :: "notification \<Rightarrow> ref_set" where
+  "refs_of_ntfn' ntfn \<equiv> ntfn_q_refs_of' (ntfnObj ntfn)
+                          \<union> get_refs NTFNBound (ntfnBoundTCB ntfn)
+                          \<union> get_refs NTFNSchedContext (ntfnSc ntfn)"
 
-definition refs_of' :: "kernel_object \<Rightarrow> (obj_ref \<times> reftype) set" where
-  "refs_of' ko \<equiv> case ko of
-     (KOTCB tcb)           => tcb_st_refs_of' (tcbState tcb) \<union> tcb_bound_refs' (tcbBoundNotification tcb)
-   | (KOEndpoint ep)       => ep_q_refs_of' ep
-   | (KONotification ntfn) => ntfn_q_refs_of' (ntfnObj ntfn) \<union> ntfn_bound_refs' (ntfnBoundTCB ntfn)
-   | _                     => {}"
+definition refs_of_sc' :: "sched_context \<Rightarrow> ref_set" where
+  "refs_of_sc' sc \<equiv> get_refs SCNtfn (scNtfn sc)
+                          \<union> get_refs SCTcb (scTCB sc)
+                          \<union> get_refs SCYieldFrom (scYieldFrom sc)
+                          \<union> get_refs SCReply (scReply sc)"
 
-definition state_refs_of' :: "kernel_state \<Rightarrow> obj_ref \<Rightarrow> (obj_ref \<times> reftype) set" where
-  "state_refs_of' s \<equiv> \<lambda>x.
-     case ksPSpace s x of
-       None \<Rightarrow> {}
-     | Some ko \<Rightarrow> if is_aligned x (objBitsKO ko) \<and> ps_clear x (objBitsKO ko) s
-                  then refs_of' ko else {}"
+definition refs_of_reply' :: "reply \<Rightarrow> ref_set" where
+  "refs_of_reply' r \<equiv> get_refs ReplySchedContext (replySC r)
+                          \<union> get_refs ReplyTCB (replyTCB r)"
+
+definition list_refs_of_reply' :: "reply \<Rightarrow> ref_set" where
+  "list_refs_of_reply' r = get_refs ReplyNext (replyNext_of r) \<union> get_refs ReplyPrev (replyPrev r)"
+
+abbreviation list_refs_of_replies_opt' :: "kernel_state \<Rightarrow> obj_ref \<Rightarrow> ref_set option" where
+  "list_refs_of_replies_opt' s \<equiv> replies_of' s ||> list_refs_of_reply'"
+
+abbreviation list_refs_of_replies' :: "kernel_state \<Rightarrow> obj_ref \<Rightarrow> ref_set" where
+  "list_refs_of_replies' s \<equiv> map_set (list_refs_of_replies_opt' s)"
+
+lemmas list_refs_of_replies'_def = map_set_def
+
+lemmas refs_of'_defs[simp] = refs_of_tcb'_def refs_of_ntfn'_def refs_of_sc'_def refs_of_reply'_def
+
+definition refs_of' :: "kernel_object \<Rightarrow> ref_set" where
+  "refs_of' x \<equiv> case x of
+    KOTCB tcb           => refs_of_tcb' tcb
+  | KOEndpoint ep       => ep_q_refs_of' ep
+  | KONotification ntfn => refs_of_ntfn' ntfn
+  | KOSchedContext sc   => refs_of_sc' sc
+  | KOReply r           => refs_of_reply' r
+  | _                   => {}"
+
+definition state_refs_of' :: "kernel_state \<Rightarrow> obj_ref \<Rightarrow> ref_set" where
+ "state_refs_of' s \<equiv> \<lambda>x. case ksPSpace s x of
+                            None \<Rightarrow> {}
+                          | Some ko \<Rightarrow>
+                              if is_aligned x (objBitsKO ko) \<and> ps_clear x (objBitsKO ko) s
+                                 \<and> objBitsKO ko < word_bits
+                              then refs_of' ko
+                              else {}"
+
+defs sym_refs_asrt_def:
+  "sym_refs_asrt \<equiv> \<lambda>s. sym_refs (state_refs_of' s)"
+
+definition live_sc' :: "sched_context \<Rightarrow> bool" where
+  "live_sc' sc \<equiv> bound (scTCB sc) \<and> scTCB sc \<noteq> Some idle_thread_ptr
+                  \<or> bound (scYieldFrom sc) \<or> bound (scNtfn sc) \<or> scReply sc \<noteq> None"
+
+definition live_ntfn' :: "notification \<Rightarrow> bool" where
+  "live_ntfn' ntfn \<equiv> bound (ntfnBoundTCB ntfn) \<or> bound (ntfnSc ntfn)
+                      \<or> (\<exists>ts. ntfnObj ntfn = WaitingNtfn ts)"
+
+definition live_reply' :: "reply \<Rightarrow> bool" where
+  "live_reply' reply \<equiv> bound (replyTCB reply) \<or> bound (replyNext reply) \<or> bound (replyPrev reply)"
 
 fun live' :: "kernel_object \<Rightarrow> bool" where
   "live' (KOTCB tcb) =
      (bound (tcbBoundNotification tcb) \<or>
-     (tcbState tcb \<noteq> Inactive \<and> tcbState tcb \<noteq> IdleThreadState) \<or>  tcbQueued tcb)"
+      bound (tcbSchedContext tcb) \<and> tcbSchedContext tcb \<noteq> Some idle_sc_ptr \<or>
+      bound (tcbYieldTo tcb) \<or>
+      tcbState tcb \<noteq> Inactive \<and> tcbState tcb \<noteq> IdleThreadState \<or>
+      tcbQueued tcb)"
 | "live' (KOEndpoint ep)       = (ep \<noteq> IdleEP)"
-| "live' (KONotification ntfn) = (bound (ntfnBoundTCB ntfn) \<or> (\<exists>ts. ntfnObj ntfn = WaitingNtfn ts))"
+| "live' (KONotification ntfn) = live_ntfn' ntfn"
+| "live' (KOSchedContext sc)   = live_sc' sc"
+| "live' (KOReply r)           = live_reply' r"
 | "live' _                     = False"
 
 fun zobj_refs' :: "capability \<Rightarrow> obj_ref set" where
   "zobj_refs' (EndpointCap r _ _ _ _ _)  = {r}"
 | "zobj_refs' (NotificationCap r _ _ _)  = {r}"
 | "zobj_refs' (ThreadCap r)              = {r}"
+| "zobj_refs' (SchedContextCap r _)      = {r}"
+| "zobj_refs' (ReplyCap r _)             = {r}"
 | "zobj_refs' _                          = {}"
 
 definition ex_nonz_cap_to' :: "obj_ref \<Rightarrow> kernel_state \<Rightarrow> bool" where
@@ -212,7 +398,6 @@ fun cte_refs' :: "capability \<Rightarrow> obj_ref \<Rightarrow> obj_ref set" wh
 | "cte_refs' (Zombie ref _ n) x        = (\<lambda>x. ref + (x << cteSizeBits)) ` {0 ..< of_nat n}"
 | "cte_refs' (IRQHandlerCap irq) x     = {x + (ucast irq << cteSizeBits)}"
 | "cte_refs' _ _                       = {}"
-
 
 abbreviation irq_node' :: "kernel_state \<Rightarrow> obj_ref" where
   "irq_node' s \<equiv> intStateIRQNode (ksInterruptState s)"
@@ -256,8 +441,13 @@ primrec capBits :: "capability \<Rightarrow> nat" where
 | "capBits (Zombie _ z _)            = zBits z"
 | "capBits (IRQControlCap)           = 0"
 | "capBits (IRQHandlerCap _)         = 0"
-| "capBits (ReplyCap _ _ _)          = objBits (undefined :: tcb)"
+| "capBits (ReplyCap tcb m)          = objBits (undefined :: reply)"
+| "capBits (SchedContextCap sc n)    = n"
+| "capBits SchedControlCap           = 0"
 | "capBits (ArchObjectCap x)         = acapBits x"
+
+lemmas objBits_defs =
+  tcbBlockSizeBits_def epSizeBits_def ntfnSizeBits_def cteSizeBits_def replySizeBits_def
 
 definition capAligned :: "capability \<Rightarrow> bool" where
   "capAligned c \<equiv> is_aligned (capUntypedPtr c) (capBits c) \<and> capBits c < word_bits"
@@ -279,6 +469,9 @@ primrec zombieCTEs :: "zombie_type \<Rightarrow> nat" where
 | "zombieCTEs (ZombieCNode n) = 2 ^ n"
 
 context begin interpretation Arch .
+
+abbreviation sc_at'_n :: "nat \<Rightarrow> obj_ref \<Rightarrow> kernel_state \<Rightarrow> bool" where
+  "sc_at'_n n \<equiv> ko_wp_at' (\<lambda>ko. koTypeOf ko = SchedContextT \<and> objBitsKO ko = n)"
 
 definition page_table_at' :: "obj_ref \<Rightarrow> kernel_state \<Rightarrow> bool" where
  "page_table_at' p \<equiv> \<lambda>s.
@@ -354,9 +547,12 @@ where valid_cap'_def:
       bits \<noteq> 0 \<and> bits + guard_sz \<le> word_bits \<and> guard && mask guard_sz = guard \<and>
       (\<forall>addr. real_cte_at' (r + 2^cteSizeBits * (addr && mask bits)) s)
   | ThreadCap r \<Rightarrow> tcb_at' r s
-  | ReplyCap r m x \<Rightarrow> tcb_at' r s
+  | ReplyCap r m \<Rightarrow> reply_at' r s
   | IRQControlCap \<Rightarrow> True
   | IRQHandlerCap irq \<Rightarrow> irq \<le> maxIRQ \<and> irq \<noteq> irqInvalid
+  | SchedControlCap \<Rightarrow> True
+  | SchedContextCap sc n \<Rightarrow> sc_at'_n n sc s
+             \<and> minSchedContextBits \<le> n \<and> n \<le> maxUntypedSizeBits
   | Zombie r b n \<Rightarrow> n \<le> zombieCTEs b \<and> zBits b < word_bits
                     \<and> (case b of ZombieTCB \<Rightarrow> tcb_at' r s | ZombieCNode n \<Rightarrow> n \<noteq> 0
                     \<and> (\<forall>addr. real_cte_at' (r + 2^cteSizeBits * (addr && mask n)) s))
@@ -369,20 +565,33 @@ abbreviation (input) valid_cap'_syn ::
 definition valid_cte' :: "cte \<Rightarrow> kernel_state \<Rightarrow> bool" where
   "valid_cte' cte s \<equiv> s \<turnstile>' (cteCap cte)"
 
+definition valid_bound_obj' ::
+  "(machine_word \<Rightarrow> kernel_state \<Rightarrow> bool) \<Rightarrow> machine_word option \<Rightarrow> kernel_state \<Rightarrow> bool" where
+  "valid_bound_obj' f p_opt s \<equiv> case p_opt of None \<Rightarrow> True | Some p \<Rightarrow> f p s"
+
+abbreviation valid_bound_ntfn' :: "obj_ref option \<Rightarrow> kernel_state \<Rightarrow> bool" where
+  "valid_bound_ntfn' \<equiv> valid_bound_obj' ntfn_at'"
+
+abbreviation valid_bound_tcb' :: "obj_ref option \<Rightarrow> kernel_state \<Rightarrow> bool" where
+  "valid_bound_tcb' \<equiv> valid_bound_obj' tcb_at'"
+
+abbreviation valid_bound_sc' :: "obj_ref option \<Rightarrow> kernel_state \<Rightarrow> bool" where
+  "valid_bound_sc' \<equiv> valid_bound_obj' sc_at'"
+
+abbreviation valid_bound_reply' :: "obj_ref option \<Rightarrow> kernel_state \<Rightarrow> bool" where
+  "valid_bound_reply' \<equiv> valid_bound_obj' reply_at'"
+
 definition valid_tcb_state' :: "thread_state \<Rightarrow> kernel_state \<Rightarrow> bool" where
   "valid_tcb_state' ts s \<equiv> case ts of
-    BlockedOnReceive ref a \<Rightarrow> ep_at' ref s
-  | BlockedOnSend ref a b d c \<Rightarrow> ep_at' ref s
-  | BlockedOnNotification ref \<Rightarrow> ntfn_at' ref s
+    BlockedOnReceive ref _ rep \<Rightarrow> ep_at' ref s \<and> valid_bound_reply' rep s
+  | BlockedOnSend ref _ _ _ _  \<Rightarrow> ep_at' ref s
+  | BlockedOnNotification ref  \<Rightarrow> ntfn_at' ref s
+  | BlockedOnReply r \<Rightarrow>  valid_bound_reply' r s
   | _ \<Rightarrow> True"
 
 definition valid_ipc_buffer_ptr' :: "machine_word \<Rightarrow> kernel_state \<Rightarrow> bool" where
   "valid_ipc_buffer_ptr' a s \<equiv>
      is_aligned a msg_align_bits \<and> typ_at' UserDataT (a && ~~ mask pageBits) s"
-
-definition valid_bound_ntfn' :: "machine_word option \<Rightarrow> kernel_state \<Rightarrow> bool" where
-  "valid_bound_ntfn' ntfn_opt s \<equiv>
-     case ntfn_opt of None \<Rightarrow> True | Some a \<Rightarrow> ntfn_at' a s"
 
 definition is_device_frame_cap' :: "capability \<Rightarrow> bool" where
   "is_device_frame_cap' cap \<equiv> case cap of ArchObjectCap (FrameCap _ _ _ dev _) \<Rightarrow> dev | _ \<Rightarrow> False"
@@ -402,28 +611,51 @@ definition valid_ep' :: "Structures_H.endpoint \<Rightarrow> kernel_state \<Righ
    | SendEP ts \<Rightarrow> (ts \<noteq> [] \<and> (\<forall>t \<in> set ts. tcb_at' t s) \<and> distinct ts)
    | RecvEP ts \<Rightarrow> (ts \<noteq> [] \<and> (\<forall>t \<in> set ts. tcb_at' t s) \<and> distinct ts)"
 
-
-definition valid_bound_tcb' :: "machine_word option \<Rightarrow> kernel_state \<Rightarrow> bool" where
-  "valid_bound_tcb' tcb_opt s \<equiv> case tcb_opt of None \<Rightarrow> True | Some t \<Rightarrow> tcb_at' t s"
-
-definition valid_ntfn' :: "Structures_H.notification \<Rightarrow> kernel_state \<Rightarrow> bool" where
+definition valid_ntfn' :: "notification \<Rightarrow> kernel_state \<Rightarrow> bool" where
   "valid_ntfn' ntfn s \<equiv> (case ntfnObj ntfn of
     IdleNtfn \<Rightarrow> True
   | WaitingNtfn ts \<Rightarrow>
-      (ts \<noteq> [] \<and> (\<forall>t \<in> set ts. tcb_at' t s) \<and> distinct ts
-     \<and> (case ntfnBoundTCB ntfn of Some tcb \<Rightarrow> ts = [tcb] | _ \<Rightarrow> True))
+      ts \<noteq> [] \<and> (\<forall>t \<in> set ts. tcb_at' t s) \<and> distinct ts
+      \<and> (case ntfnBoundTCB ntfn of Some tcb \<Rightarrow> ts = [tcb] | _ \<Rightarrow> True)
   | ActiveNtfn b \<Rightarrow> True)
-  \<and> valid_bound_tcb' (ntfnBoundTCB ntfn) s"
+  \<and> valid_bound_tcb' (ntfnBoundTCB ntfn) s
+  \<and> valid_bound_sc' (ntfnSc ntfn) s"
+
+definition valid_sched_context' :: "sched_context \<Rightarrow> kernel_state \<Rightarrow> bool" where
+  "valid_sched_context' sc s \<equiv>
+     valid_bound_ntfn' (scNtfn sc) s
+     \<and> valid_bound_tcb' (scTCB sc) s
+     \<and> valid_bound_tcb' (scYieldFrom sc) s
+     \<and> valid_bound_reply' (scReply sc) s
+     \<and> MIN_REFILLS \<le> length (scRefills sc)
+     \<and> scRefillMax sc \<le> length (scRefills sc)
+     \<and> (0 < scRefillMax sc \<longrightarrow> scRefillHead sc < scRefillMax sc
+                               \<and> scRefillCount sc \<le> scRefillMax sc
+                               \<and> 0 < scRefillCount sc)
+     \<and> length (scRefills sc) = refillAbsoluteMax' (scBitsFromRefillLength' (length (scRefills sc)))"
+
+definition valid_reply' :: "reply \<Rightarrow> kernel_state \<Rightarrow> bool" where
+  "valid_reply' reply s \<equiv>
+     valid_bound_tcb' (replyTCB reply) s
+     \<and> valid_bound_sc' (replySC reply) s
+     \<and> valid_bound_reply' (replyPrev reply) s
+     \<and> valid_bound_reply' (replyNext_of reply) s"
 
 definition valid_mapping' :: "machine_word \<Rightarrow> vmpage_size \<Rightarrow> kernel_state \<Rightarrow> bool" where
   "valid_mapping' x sz s \<equiv> is_aligned x (pageBitsForSize sz) \<and> ptrFromPAddr x \<noteq> 0"
 
-definition
-  valid_obj' :: "Structures_H.kernel_object \<Rightarrow> kernel_state \<Rightarrow> bool"
-where
+definition sc_size_bounds :: "nat \<Rightarrow> bool" where
+  "sc_size_bounds us \<equiv> minSchedContextBits \<le> us \<and> us \<le> maxUntypedSizeBits"
+
+definition valid_sched_context_size' :: "sched_context \<Rightarrow> bool" where
+  "valid_sched_context_size' sc \<equiv> sc_size_bounds (objBits sc)"
+
+definition valid_obj' :: "kernel_object \<Rightarrow> kernel_state \<Rightarrow> bool" where
   "valid_obj' ko s \<equiv> case ko of
     KOEndpoint endpoint \<Rightarrow> valid_ep' endpoint s
   | KONotification notification \<Rightarrow> valid_ntfn' notification s
+  | KOSchedContext sc \<Rightarrow> valid_sched_context' sc s \<and> valid_sched_context_size' sc
+  | KOReply reply \<Rightarrow> valid_reply' reply s
   | KOKernelData \<Rightarrow> False
   | KOUserData \<Rightarrow> True
   | KOUserDataDevice \<Rightarrow> True
@@ -442,6 +674,9 @@ definition
 where
  "pspace_canonical' s \<equiv> \<forall>p \<in> dom (ksPSpace s). canonical_address p"
 
+definition pspace_bounded' :: "kernel_state \<Rightarrow> bool" where
+  "pspace_bounded' s \<equiv> \<forall>x \<in> dom (ksPSpace s). objBitsKO (the (ksPSpace s x)) < word_bits"
+
 definition
   pspace_in_kernel_mappings' :: "kernel_state \<Rightarrow> bool"
 where
@@ -458,6 +693,18 @@ definition
 where
   "valid_objs' s \<equiv> \<forall>obj \<in> ran (ksPSpace s). valid_obj' obj s"
 
+definition valid_obj_size' :: "kernel_object \<Rightarrow> kernel_state \<Rightarrow> bool" where
+  "valid_obj_size' ko s \<equiv> case ko of
+    KOSchedContext sc \<Rightarrow> valid_sched_context_size' sc
+  | _ \<Rightarrow> True"
+
+definition valid_objs_size' :: "kernel_state \<Rightarrow> bool" where
+  "valid_objs_size' s \<equiv> \<forall>obj \<in> ran (ksPSpace s). valid_obj_size' obj s"
+
+lemma valid_objs'_valid_objs_size':
+  "valid_objs' s \<Longrightarrow> valid_objs_size' s"
+  by (clarsimp simp: valid_objs'_def valid_objs_size'_def valid_obj'_def valid_obj_size'_def)
+     (fastforce split: kernel_object.splits)
 
 type_synonym cte_heap = "machine_word \<Rightarrow> cte option"
 
@@ -546,12 +793,14 @@ where
 | "capClass (UntypedCap d p n f)               = PhysicalClass"
 | "capClass (EndpointCap ref badge s r g gr)   = PhysicalClass"
 | "capClass (NotificationCap ref badge s r)    = PhysicalClass"
+| "capClass (SchedContextCap _ _)              = PhysicalClass"
 | "capClass (CNodeCap ref bits g gs)           = PhysicalClass"
 | "capClass (ThreadCap ref)                    = PhysicalClass"
 | "capClass (Zombie r b n)                     = PhysicalClass"
 | "capClass (IRQControlCap)                    = IRQClass"
+| "capClass (SchedControlCap)                  = SchedControlClass"
 | "capClass (IRQHandlerCap irq)                = IRQClass"
-| "capClass (ReplyCap tcb m g)                 = ReplyClass tcb"
+| "capClass (ReplyCap tcb m)                   = PhysicalClass"
 | "capClass (ArchObjectCap cap)                = acapClass cap"
 
 definition
@@ -686,13 +935,6 @@ where
  "distinct_zombies m \<equiv> distinct_zombie_caps (option_map cteCap \<circ> m)"
 
 definition
-  reply_masters_rvk_fb :: "cte_heap \<Rightarrow> bool"
-where
- "reply_masters_rvk_fb ctes \<equiv> \<forall>cte \<in> ran ctes.
-        isReplyCap (cteCap cte) \<and> capReplyMaster (cteCap cte)
-    \<longrightarrow> mdbRevocable (cteMDBNode cte) \<and> mdbFirstBadged (cteMDBNode cte)"
-
-definition
   valid_mdb_ctes :: "cte_heap \<Rightarrow> bool"
 where
   "valid_mdb_ctes \<equiv> \<lambda>m. valid_dlist m \<and> no_0 m \<and> mdb_chain_0 m \<and>
@@ -700,7 +942,7 @@ where
                         mdb_chunked m \<and> untyped_mdb' m \<and>
                         untyped_inc' m \<and> valid_nullcaps m \<and>
                         ut_revocable' m \<and> class_links m \<and> distinct_zombies m
-                        \<and> irq_control m \<and> reply_masters_rvk_fb m"
+                        \<and> irq_control m"
 
 definition
   valid_mdb' :: "kernel_state \<Rightarrow> bool"
@@ -710,28 +952,41 @@ where
 definition
   "no_0_obj' \<equiv> \<lambda>s. ksPSpace s 0 = None"
 
+abbreviation is_reply_linked :: "obj_ref \<Rightarrow> kernel_state \<Rightarrow> bool" where
+  "is_reply_linked rptr s \<equiv> replyNexts_of s rptr \<noteq> None \<or> replyPrevs_of s rptr \<noteq> None"
+
+definition valid_replies'_except :: "obj_ref set \<Rightarrow> kernel_state \<Rightarrow> bool" where
+  "valid_replies'_except RS s \<equiv>
+     \<forall>rptr. rptr \<notin> RS \<and> is_reply_linked rptr s
+            \<longrightarrow> (\<exists>tptr. replyTCBs_of s rptr = Some tptr
+                        \<and> st_tcb_at' ((=) (BlockedOnReply (Some rptr))) tptr s)"
+
+definition [simplified empty_iff simp_thms valid_replies'_except_def]:
+  "valid_replies' s \<equiv> valid_replies'_except {} s"
+
+defs valid_replies'_sc_asrt_def:
+  "valid_replies'_sc_asrt \<equiv> \<lambda>rptr s.
+     replySCs_of s rptr \<noteq> None
+       \<longrightarrow> (\<exists>tptr. replyTCBs_of s rptr = Some tptr
+                   \<and> st_tcb_at' ((=) (BlockedOnReply (Some rptr))) tptr s)"
+
 definition
   valid_pspace' :: "kernel_state \<Rightarrow> bool"
 where
   "valid_pspace' \<equiv> valid_objs' and
+                   valid_replies' and
                    pspace_aligned' and
                    pspace_canonical' and
                    pspace_in_kernel_mappings' and
                    pspace_distinct' and
+                   pspace_bounded' and
                    no_0_obj' and
                    valid_mdb'"
 
-primrec
-  runnable' :: "Structures_H.thread_state \<Rightarrow> bool"
-where
-  "runnable' (Structures_H.Running)                 = True"
-| "runnable' (Structures_H.Inactive)                = False"
-| "runnable' (Structures_H.Restart)                 = True"
-| "runnable' (Structures_H.IdleThreadState)         = False"
-| "runnable' (Structures_H.BlockedOnReceive a b)    = False"
-| "runnable' (Structures_H.BlockedOnReply)          = False"
-| "runnable' (Structures_H.BlockedOnSend a b c d e) = False"
-| "runnable' (Structures_H.BlockedOnNotification x) = False"
+fun runnable' :: "thread_state \<Rightarrow> bool" where
+  "runnable' Running = True"
+| "runnable' Restart = True"
+| "runnable' _       = False"
 
 definition
   inQ :: "domain \<Rightarrow> priority \<Rightarrow> tcb \<Rightarrow> bool"
@@ -747,13 +1002,16 @@ where
                      \<and> ksReadyQueuesL2Bitmap s (d, invertL1Index (prioToL1Index p))
                          !! unat (p && mask wordRadix)"
 
-definition
-  valid_queues_no_bitmap :: "kernel_state \<Rightarrow> bool"
-where
+definition valid_queues_no_bitmap :: "kernel_state \<Rightarrow> bool" where
  "valid_queues_no_bitmap \<equiv> \<lambda>s.
-   (\<forall>d p. (\<forall>t \<in> set (ksReadyQueues s (d, p)). obj_at' (inQ d p and runnable' \<circ> tcbState) t s)
-    \<and>  distinct (ksReadyQueues s (d, p))
-    \<and> (d > maxDomain \<or> p > maxPriority \<longrightarrow> ksReadyQueues s (d,p) = []))"
+   \<forall>d p. (\<forall>t \<in> set (ksReadyQueues s (d, p)). obj_at' (inQ d p) t s)
+          \<and> (d > maxDomain \<or> p > maxPriority \<longrightarrow> ksReadyQueues s (d,p) = [])"
+
+defs ready_qs_runnable_def:
+  "ready_qs_runnable \<equiv> \<lambda>s. \<forall>d p. \<forall>t \<in> set (ksReadyQueues s (d, p)). st_tcb_at' runnable' t s"
+
+definition notQueued :: "obj_ref \<Rightarrow> kernel_state \<Rightarrow> bool" where
+  "notQueued t s \<equiv> (\<forall>d p. t \<notin> set (ksReadyQueues s (d, p)))"
 
 definition
   (* A priority is used as a two-part key into the bitmap structure. If an L2 bitmap entry
@@ -799,10 +1057,28 @@ where
 lemmas bitmapQ_defs = valid_bitmapQ_def valid_bitmapQ_except_def bitmapQ_def
                        bitmapQ_no_L2_orphans_def bitmapQ_no_L1_orphans_def
 
+(* valid_queues is too strong sometimes *)
+definition valid_inQ_queues :: "kernel_state \<Rightarrow> bool" where
+  "valid_inQ_queues \<equiv> \<lambda>s. \<forall>d p. \<forall>t\<in>set (ksReadyQueues s (d, p)). obj_at' (inQ d p) t s"
+
+(* when in the middle of updates, a particular queue might not be entirely valid *)
+definition valid_inQ_queues_except :: "obj_ref \<Rightarrow> kernel_state \<Rightarrow> bool" where
+ "valid_inQ_queues_except t'
+   \<equiv> \<lambda>s. \<forall>d p. \<forall>t \<in> set (ksReadyQueues s (d, p)). t \<noteq> t' \<longrightarrow> obj_at' (inQ d p) t s"
+
 definition
   valid_queues' :: "kernel_state \<Rightarrow> bool"
 where
  "valid_queues' \<equiv> \<lambda>s. \<forall>d p t. obj_at' (inQ d p) t s \<longrightarrow> t \<in> set (ksReadyQueues s (d, p))"
+
+definition valid_release_queue :: "kernel_state \<Rightarrow> bool" where
+ "valid_release_queue \<equiv> \<lambda>s. \<forall>t. t \<in> set (ksReleaseQueue s) \<longrightarrow> obj_at' (tcbInReleaseQueue) t s"
+
+definition valid_release_queue' :: "kernel_state \<Rightarrow> bool" where
+ "valid_release_queue' \<equiv> \<lambda>s. \<forall>t. obj_at' (tcbInReleaseQueue) t s \<longrightarrow> t \<in> set (ksReleaseQueue s)"
+
+abbreviation valid_release_queue_iff :: "kernel_state \<Rightarrow> bool" where
+  "valid_release_queue_iff \<equiv> valid_release_queue and valid_release_queue'"
 
 definition tcb_in_cur_domain' :: "machine_word \<Rightarrow> kernel_state \<Rightarrow> bool" where
   "tcb_in_cur_domain' t \<equiv> \<lambda>s. obj_at' (\<lambda>tcb. ksCurDomain s = tcbDomain tcb) t s"
@@ -812,12 +1088,15 @@ definition
   "ct_idle_or_in_cur_domain' \<equiv> \<lambda>s. ksSchedulerAction s = ResumeCurrentThread \<longrightarrow>
     ksCurThread s = ksIdleThread s \<or> tcb_in_cur_domain' (ksCurThread s) s"
 
-definition
+definition ct_in_state' :: "(thread_state \<Rightarrow> bool) \<Rightarrow> kernel_state \<Rightarrow> bool" where
  "ct_in_state' test \<equiv> \<lambda>s. st_tcb_at' test (ksCurThread s) s"
 
 definition
  "ct_not_inQ \<equiv> \<lambda>s. ksSchedulerAction s = ResumeCurrentThread
                      \<longrightarrow> obj_at' (Not \<circ> tcbQueued) (ksCurThread s) s"
+
+defs ct_not_inQ_asrt_def:
+  "ct_not_inQ_asrt \<equiv> \<lambda>s. ct_not_inQ s"
 
 abbreviation
   "idle' \<equiv> \<lambda>st. st = Structures_H.IdleThreadState"
@@ -825,12 +1104,19 @@ abbreviation
 abbreviation
   "activatable' st \<equiv> runnable' st \<or> idle' st"
 
+defs rct_imp_activatable'_asrt_def:
+  "rct_imp_activatable'_asrt \<equiv> \<lambda>s. ksSchedulerAction s = ResumeCurrentThread \<longrightarrow>
+                                         ct_in_state' activatable' s"
+
 primrec
   sch_act_wf :: "scheduler_action \<Rightarrow> kernel_state \<Rightarrow> bool"
 where
   "sch_act_wf ResumeCurrentThread = ct_in_state' activatable'"
 | "sch_act_wf ChooseNewThread     = \<top>"
 | "sch_act_wf (SwitchToThread t)  = (\<lambda>s. st_tcb_at' runnable' t s \<and> tcb_in_cur_domain' t s)"
+
+defs sch_act_wf_asrt_def:
+  "sch_act_wf_asrt \<equiv> \<lambda>s. sch_act_wf (ksSchedulerAction s) s"
 
 definition sch_act_simple :: "kernel_state \<Rightarrow> bool" where
   "sch_act_simple \<equiv> \<lambda>s. (ksSchedulerAction s = ResumeCurrentThread) \<or>
@@ -842,19 +1128,41 @@ definition sch_act_sane :: "kernel_state \<Rightarrow> bool" where
 abbreviation
   "sch_act_not t \<equiv> \<lambda>s. ksSchedulerAction s \<noteq> SwitchToThread t"
 
-definition idle_tcb'_2 :: "Structures_H.thread_state \<times> machine_word option \<Rightarrow> bool" where
-  "idle_tcb'_2 \<equiv> \<lambda>(st, ntfn_opt). (idle' st \<and> ntfn_opt = None)"
+definition idle_tcb'_2 ::
+  "thread_state \<times> obj_ref option \<times> obj_ref option \<times> obj_ref option \<Rightarrow> bool"
+  where
+  "idle_tcb'_2 \<equiv> \<lambda>(st, ntfn_opt, sc_opt, yt_opt).
+                    (idle' st \<and> ntfn_opt = None \<and> sc_opt = Some idle_sc_ptr \<and> yt_opt = None)"
 
-abbreviation
-  "idle_tcb' tcb \<equiv> idle_tcb'_2 (tcbState tcb, tcbBoundNotification tcb)"
+abbreviation  idle_tcb' :: "tcb \<Rightarrow> bool" where
+  "idle_tcb' tcb \<equiv>
+      idle_tcb'_2 (tcbState tcb, tcbBoundNotification tcb, tcbSchedContext tcb, tcbYieldTo tcb)"
 
 lemmas idle_tcb'_def = idle_tcb'_2_def
 
+abbreviation idle_sc' :: "sched_context \<Rightarrow> bool" where
+  "idle_sc' sc \<equiv>
+      scPeriod sc = 0
+      \<and> scTCB sc = Some idle_thread_ptr
+      \<and> scNtfn sc = None
+      \<and> scRefillMax sc = MIN_REFILLS
+      \<and> scBadge sc = 0
+      \<and> scYieldFrom sc = None
+      \<and> scReply sc = None"
+
+abbreviation idle_sc_at' :: "obj_ref \<Rightarrow> kernel_state \<Rightarrow> bool" where
+  "idle_sc_at' \<equiv> obj_at' idle_sc'"
+
 definition valid_idle' :: "kernel_state \<Rightarrow> bool" where
-  "valid_idle' \<equiv> \<lambda>s. obj_at' idle_tcb' (ksIdleThread s) s \<and> idle_thread_ptr = ksIdleThread s"
+  "valid_idle' \<equiv> \<lambda>s. obj_at' idle_tcb' (ksIdleThread s) s
+                      \<and> idle_sc_at' idle_sc_ptr s
+                      \<and> idle_thread_ptr = ksIdleThread s"
+
+defs valid_idle'_asrt_def:
+  "valid_idle'_asrt \<equiv> \<lambda>s. valid_idle' s"
 
 lemma valid_idle'_tcb_at':
-  "valid_idle' s \<Longrightarrow> obj_at' idle_tcb' (ksIdleThread s) s"
+  "valid_idle' s \<Longrightarrow> obj_at' idle_tcb' (ksIdleThread s) s \<and> idle_sc_at' idle_sc_ptr s"
   by (clarsimp simp: valid_idle'_def)
 
 definition valid_irq_node' :: "machine_word \<Rightarrow> kernel_state \<Rightarrow> bool" where
@@ -872,7 +1180,7 @@ definition
   global_refs' :: "kernel_state \<Rightarrow> obj_ref set"
 where
   "global_refs' \<equiv> \<lambda>s.
-   {ksIdleThread s} \<union>
+   {ksIdleThread s, idle_sc_ptr} \<union>
    (\<Union>l. (\<Union> (table_refs' ` set (riscvKSGlobalPTs (ksArchState s) l)))) \<union>
    range (\<lambda>irq :: irq. irq_node' s + (ucast irq << cteSizeBits))"
 
@@ -939,19 +1247,18 @@ definition
 abbreviation
   "untyped_ranges_zero' s \<equiv> untyped_ranges_zero_inv (cteCaps_of s) (gsUntypedZeroRanges s)"
 
-(* FIXME: this really should be a definition like the above. *)
 (* The schedule is invariant. *)
-abbreviation
+definition valid_dom_schedule' :: "kernel_state \<Rightarrow> bool" where
   "valid_dom_schedule' \<equiv>
    \<lambda>s. ksDomSchedule s \<noteq> [] \<and> (\<forall>x\<in>set (ksDomSchedule s). dschDomain x \<le> maxDomain \<and> 0 < dschLength x)
        \<and> ksDomSchedule s = ksDomSchedule (newKernelState undefined)
        \<and> ksDomScheduleIdx s < length (ksDomSchedule (newKernelState undefined))"
 
-definition valid_state' :: "kernel_state \<Rightarrow> bool" where
-  "valid_state' \<equiv> \<lambda>s. valid_pspace' s \<and> sch_act_wf (ksSchedulerAction s) s
-                      \<and> valid_queues s \<and> sym_refs (state_refs_of' s)
+definition invs' :: "kernel_state \<Rightarrow> bool" where
+  "invs' \<equiv> \<lambda>s. valid_pspace' s
+                      \<and> valid_queues s
+                      \<and> sym_refs (list_refs_of_replies' s)
                       \<and> if_live_then_nonz_cap' s \<and> if_unsafe_then_cap' s
-                      \<and> valid_idle' s
                       \<and> valid_global_refs' s \<and> valid_arch_state' s
                       \<and> valid_irq_node' (irq_node' s) s
                       \<and> valid_irq_handlers' s
@@ -959,8 +1266,8 @@ definition valid_state' :: "kernel_state \<Rightarrow> bool" where
                       \<and> valid_machine_state' s
                       \<and> irqs_masked' s
                       \<and> valid_queues' s
-                      \<and> ct_not_inQ s
-                      \<and> ct_idle_or_in_cur_domain' s
+                      \<and> valid_release_queue s
+                      \<and> valid_release_queue' s
                       \<and> pspace_domain_valid s
                       \<and> ksCurDomain s \<le> maxDomain
                       \<and> valid_dom_schedule' s
@@ -969,15 +1276,20 @@ definition valid_state' :: "kernel_state \<Rightarrow> bool" where
 definition
   "cur_tcb' s \<equiv> tcb_at' (ksCurThread s) s"
 
-definition
-  invs' :: "kernel_state \<Rightarrow> bool" where
-  "invs' \<equiv> valid_state' and cur_tcb'"
+defs cur_tcb'_asrt_def:
+  "cur_tcb'_asrt \<equiv> \<lambda>s. cur_tcb' s"
+
+defs sch_act_sane_asrt_def:
+  "sch_act_sane_asrt \<equiv> \<lambda>s. sch_act_sane s"
+
+defs ct_not_ksQ_asrt_def:
+  "ct_not_ksQ_asrt \<equiv> \<lambda>s. \<forall>pd. ksCurThread s \<notin> set (ksReadyQueues s pd)"
 
 
 subsection "Derived concepts"
 
 abbreviation
-  "awaiting_reply' ts \<equiv> ts = Structures_H.BlockedOnReply"
+  "awaiting_reply' ts \<equiv> isBlockedOnReply ts"
 
   (* x-symbol doesn't have a reverse leadsto.. *)
 definition
@@ -993,6 +1305,8 @@ definition
                     | NotificationT \<Rightarrow> injectKO (makeObject :: Structures_H.notification)
                     | CTET \<Rightarrow> injectKO (makeObject :: cte)
                     | TCBT \<Rightarrow> injectKO (makeObject :: tcb)
+                    | SchedContextT \<Rightarrow> injectKO (makeObject :: sched_context)
+                    | ReplyT \<Rightarrow> injectKO (makeObject :: reply)
                     | UserDataT \<Rightarrow> injectKO (makeObject :: user_data)
                     | UserDataDeviceT \<Rightarrow> injectKO (makeObject :: user_data_device)
                     | KernelDataT \<Rightarrow> KOKernelData
@@ -1009,11 +1323,16 @@ definition
 abbreviation
   "active' st \<equiv> st = Structures_H.Running \<or> st = Structures_H.Restart"
 
+lemma runnable_eq_active': "runnable' = active'"
+  apply (rule ext)
+  apply (case_tac st, simp_all)
+  done
+
 abbreviation
   "simple' st \<equiv> st = Structures_H.Inactive \<or>
                 st = Structures_H.Running \<or>
                 st = Structures_H.Restart \<or>
-                idle' st \<or> awaiting_reply' st"
+                idle' st"
 
 abbreviation
   "ct_active' \<equiv> ct_in_state' active'"
@@ -1021,65 +1340,9 @@ abbreviation
 abbreviation
   "ct_running' \<equiv> ct_in_state' (\<lambda>st. st = Structures_H.Running)"
 
-abbreviation(input)
- "all_invs_but_sym_refs_ct_not_inQ'
-    \<equiv> \<lambda>s. valid_pspace' s \<and> sch_act_wf (ksSchedulerAction s) s
-           \<and> valid_queues s \<and> if_live_then_nonz_cap' s \<and> if_unsafe_then_cap' s
-           \<and> valid_idle' s \<and> valid_global_refs' s \<and> valid_arch_state' s
-           \<and> valid_irq_node' (irq_node' s) s \<and> valid_irq_handlers' s
-           \<and> valid_irq_states' s \<and> irqs_masked' s \<and> valid_machine_state' s
-           \<and> cur_tcb' s \<and> valid_queues' s \<and> ct_idle_or_in_cur_domain' s
-           \<and> pspace_domain_valid s
-           \<and> ksCurDomain s \<le> maxDomain
-           \<and> valid_dom_schedule' s \<and> untyped_ranges_zero' s"
+defs ct_active'_asrt_def:
+  "ct_active'_asrt \<equiv> ct_active'"
 
-abbreviation(input)
- "all_invs_but_ct_not_inQ'
-    \<equiv> \<lambda>s. valid_pspace' s \<and> sch_act_wf (ksSchedulerAction s) s
-           \<and> valid_queues s \<and> sym_refs (state_refs_of' s)
-           \<and> if_live_then_nonz_cap' s \<and> if_unsafe_then_cap' s
-           \<and> valid_idle' s \<and> valid_global_refs' s \<and> valid_arch_state' s
-           \<and> valid_irq_node' (irq_node' s) s \<and> valid_irq_handlers' s
-           \<and> valid_irq_states' s \<and> irqs_masked' s \<and> valid_machine_state' s
-           \<and> cur_tcb' s \<and> valid_queues' s \<and> ct_idle_or_in_cur_domain' s
-           \<and> pspace_domain_valid s
-           \<and> ksCurDomain s \<le> maxDomain
-           \<and> valid_dom_schedule' s \<and> untyped_ranges_zero' s"
-
-lemma all_invs_but_sym_refs_not_ct_inQ_check':
-  "(all_invs_but_sym_refs_ct_not_inQ' and sym_refs \<circ> state_refs_of' and ct_not_inQ) = invs'"
-  by (simp add: pred_conj_def conj_commute conj_left_commute invs'_def valid_state'_def)
-
-lemma all_invs_but_not_ct_inQ_check':
-  "(all_invs_but_ct_not_inQ' and ct_not_inQ) = invs'"
-  by (simp add: pred_conj_def conj_commute conj_left_commute invs'_def valid_state'_def)
-
-definition
-  "all_invs_but_ct_idle_or_in_cur_domain'
-    \<equiv> \<lambda>s. valid_pspace' s \<and> sch_act_wf (ksSchedulerAction s) s
-           \<and> valid_queues s \<and> sym_refs (state_refs_of' s)
-           \<and> if_live_then_nonz_cap' s \<and> if_unsafe_then_cap' s
-           \<and> valid_idle' s \<and> valid_global_refs' s \<and> valid_arch_state' s
-           \<and> valid_irq_node' (irq_node' s) s \<and> valid_irq_handlers' s
-           \<and> valid_irq_states' s \<and> irqs_masked' s \<and> valid_machine_state' s
-           \<and> cur_tcb' s \<and> valid_queues' s \<and> ct_not_inQ s
-           \<and> pspace_domain_valid s
-           \<and> ksCurDomain s \<le> maxDomain
-           \<and> valid_dom_schedule' s \<and> untyped_ranges_zero' s"
-
-lemmas invs_no_cicd'_def = all_invs_but_ct_idle_or_in_cur_domain'_def
-
-lemma all_invs_but_ct_idle_or_in_cur_domain_check':
-  "(all_invs_but_ct_idle_or_in_cur_domain' and ct_idle_or_in_cur_domain') = invs'"
-  by (simp add: all_invs_but_ct_idle_or_in_cur_domain'_def pred_conj_def
-                conj_left_commute conj_commute invs'_def valid_state'_def)
-
-abbreviation (input)
-  "invs_no_cicd' \<equiv> all_invs_but_ct_idle_or_in_cur_domain'"
-
-lemma invs'_to_invs_no_cicd'_def:
-  "invs' = (all_invs_but_ct_idle_or_in_cur_domain' and ct_idle_or_in_cur_domain')"
-  by (fastforce simp: invs'_def all_invs_but_ct_idle_or_in_cur_domain'_def valid_state'_def )
 end
 
 locale mdb_next =
@@ -1123,27 +1386,19 @@ section "Lemmas"
 schematic_goal wordBits_def': "wordBits = numeral ?n" (* arch-specific consequence *)
   by (simp add: wordBits_def word_size)
 
-lemma valid_bound_ntfn'_None[simp]:
-  "valid_bound_ntfn' None = \<top>"
-  by (auto simp: valid_bound_ntfn'_def)
+lemmas valid_bound_ntfn'_def = valid_bound_obj'_def
+lemmas valid_bound_tcb'_def = valid_bound_obj'_def
+lemmas valid_bound_sc'_def = valid_bound_obj'_def
+lemmas valid_bound_reply'_def = valid_bound_obj'_def
 
-lemma valid_bound_ntfn'_Some[simp]:
-  "valid_bound_ntfn' (Some x) = ntfn_at' x"
-  by (auto simp: valid_bound_ntfn'_def)
+lemma valid_bound_obj'_None[simp]:
+  "valid_bound_obj' P None = \<top>"
+  by (auto simp: valid_bound_obj'_def)
 
-lemma valid_bound_tcb'_None[simp]:
-  "valid_bound_tcb' None = \<top>"
-  by (auto simp: valid_bound_tcb'_def)
+lemma valid_bound_obj'_Some[simp]:
+  "valid_bound_obj' P (Some x) = P x"
+  by (auto simp: valid_bound_obj'_def)
 
-lemma valid_bound_tcb'_Some[simp]:
-  "valid_bound_tcb' (Some x) = tcb_at' x"
-  by (auto simp: valid_bound_tcb'_def)
-
-lemma objBitsKO_Data:
-  "objBitsKO (if dev then KOUserDataDevice else KOUserData) = pageBits"
-  by (simp add: objBits_def objBitsKO_def word_size_def)
-
-lemmas objBits_defs = tcbBlockSizeBits_def epSizeBits_def ntfnSizeBits_def cteSizeBits_def
 lemmas untypedBits_defs = minUntypedSizeBits_def maxUntypedSizeBits_def
 lemmas objBits_simps = objBits_def objBitsKO_def word_size_def archObjSize_def
 lemmas objBits_simps' = objBits_simps objBits_defs
@@ -1169,26 +1424,25 @@ lemma ps_clear_def2:
   done
 
 lemma projectKO_stateI:
-  "fst (projectKO e s) = {(obj, s)} \<Longrightarrow> fst (projectKO e s') = {(obj, s')}"
+  "projectKO e s = Some obj \<Longrightarrow> projectKO e s' = Some obj"
   unfolding projectKO_def
-  by (auto simp: fail_def return_def valid_def split: option.splits)
+  by (auto simp: omonad_defs split: option.splits)
 
 lemma singleton_in_magnitude_check:
   "(x, s) \<in> fst (magnitudeCheck a b c s') \<Longrightarrow> \<forall>s'. fst (magnitudeCheck a b c s') = {(x, s')}"
-  by (simp add: magnitudeCheck_def when_def in_monad return_def
-         split: if_split_asm option.split_asm)
+  by (fastforce simp: read_magnitudeCheck_def magnitudeCheck_def in_monad
+               split: option.split_asm)
 
 lemma wordSizeCase_simp [simp]: "wordSizeCase a b = b"
   by (simp add: wordSizeCase_def wordBits_def word_size)
 
-lemma projectKO_eq:
-  "(fst (projectKO ko c) = {(obj, c)}) = (projectKO_opt ko = Some obj)"
-  by (simp add: projectKO_def fail_def return_def split: option.splits)
+(* FIXME RT: cleanup: with the reader monad, projectKO_eq is identical to projectKO_eq2. *)
+lemmas projectKO_eq = projectKO_eq2
 
 lemma obj_at'_def':
   "obj_at' P p s = (\<exists>ko obj. ksPSpace s p = Some ko \<and> is_aligned p (objBitsKO ko)
-                   \<and> fst (projectKO ko s) = {(obj,s)} \<and> P obj
-                   \<and> ps_clear p (objBitsKO ko) s)"
+                   \<and> projectKO ko s = Some obj \<and> P obj
+                   \<and> ps_clear p (objBitsKO ko) s \<and> objBitsKO ko < word_bits)"
   apply (simp add: obj_at'_real_def ko_wp_at'_def projectKO_eq
                    True_notin_set_replicate_conv objBits_def)
   apply fastforce
@@ -1196,22 +1450,22 @@ lemma obj_at'_def':
 
 lemma obj_at'_def:
   "obj_at' P p s \<equiv> \<exists>ko obj. ksPSpace s p = Some ko \<and> is_aligned p (objBitsKO ko)
-                   \<and> fst (projectKO ko s) = {(obj,s)} \<and> P obj
-                   \<and> ps_clear p (objBitsKO ko) s"
+                   \<and> projectKO ko s = Some obj \<and> P obj
+                   \<and> ps_clear p (objBitsKO ko) s \<and> objBitsKO ko < word_bits"
   by (simp add: obj_at'_def')
 
 lemma obj_atE' [elim?]:
   assumes objat: "obj_at' P ptr s"
   and        rl: "\<And>ko obj.
   \<lbrakk> ksPSpace s ptr = Some ko; is_aligned ptr (objBitsKO ko);
-     fst (projectKO ko s) = {(obj,s)}; P obj;
+     projectKO ko s = Some obj; P obj; objBitsKO ko < word_bits;
      ps_clear ptr (objBitsKO ko) s \<rbrakk> \<Longrightarrow> R"
   shows "R"
   using objat unfolding obj_at'_def by (auto intro!: rl)
 
 lemma obj_atI' [intro?]:
   "\<lbrakk> ksPSpace s ptr = Some ko; is_aligned ptr (objBitsKO ko);
-       fst (projectKO ko s) = {(obj, s)}; P obj;
+       projectKO ko s = Some obj; P obj; objBitsKO ko < word_bits;
        ps_clear ptr (objBitsKO ko) s \<rbrakk>
   \<Longrightarrow> obj_at' P ptr s"
   unfolding obj_at'_def by (auto)
@@ -1221,48 +1475,18 @@ lemma cte_at'_def:
   "cte_at' p s \<equiv> \<exists>cte::cte. fst (getObject p s) = {(cte,s)}"
   by (simp add: cte_wp_at'_def)
 
-
 lemma tcb_cte_cases_simps[simp]:
   "tcb_cte_cases 0  = Some (tcbCTable, tcbCTable_update)"
   "tcb_cte_cases 32 = Some (tcbVTable, tcbVTable_update)"
-  "tcb_cte_cases 64 = Some (tcbReply, tcbReply_update)"
-  "tcb_cte_cases 96 = Some (tcbCaller, tcbCaller_update)"
-  "tcb_cte_cases 128 = Some (tcbIPCBufferFrame, tcbIPCBufferFrame_update)"
+  "tcb_cte_cases 64 = Some (tcbIPCBufferFrame, tcbIPCBufferFrame_update)"
+  "tcb_cte_cases 96 = Some (tcbFaultHandler, tcbFaultHandler_update)"
+  "tcb_cte_cases 128 = Some (tcbTimeoutHandler, tcbTimeoutHandler_update)"
   by (simp add: tcb_cte_cases_def cteSizeBits_def)+
 
-lemma refs_of'_simps[simp]:
- "refs_of' (KOTCB tcb)           = tcb_st_refs_of' (tcbState tcb) \<union> tcb_bound_refs' (tcbBoundNotification tcb)"
- "refs_of' (KOCTE cte)           = {}"
- "refs_of' (KOEndpoint ep)       = ep_q_refs_of' ep"
- "refs_of' (KONotification ntfn)     = ntfn_q_refs_of' (ntfnObj ntfn) \<union> ntfn_bound_refs' (ntfnBoundTCB ntfn)"
- "refs_of' (KOUserData)          = {}"
- "refs_of' (KOUserDataDevice)          = {}"
- "refs_of' (KOKernelData)        = {}"
- "refs_of' (KOArch ako)          = {}"
-  by (auto simp: refs_of'_def)
-
-lemma tcb_st_refs_of'_simps[simp]:
- "tcb_st_refs_of' (Running)                  = {}"
- "tcb_st_refs_of' (Inactive)                 = {}"
- "tcb_st_refs_of' (Restart)                  = {}"
- "tcb_st_refs_of' (BlockedOnReceive x'' a')  = {(x'', TCBBlockedRecv)}"
- "tcb_st_refs_of' (BlockedOnSend x a b c d)  = {(x, TCBBlockedSend)}"
- "tcb_st_refs_of' (BlockedOnNotification x') = {(x', TCBSignal)}"
- "tcb_st_refs_of' (BlockedOnReply)           = {}"
- "tcb_st_refs_of' (IdleThreadState)          = {}"
-  by (auto simp: tcb_st_refs_of'_def)
-
-lemma ep_q_refs_of'_simps[simp]:
- "ep_q_refs_of'  IdleEP    = {}"
- "ep_q_refs_of' (RecvEP q) = set q \<times> {EPRecv}"
- "ep_q_refs_of' (SendEP q) = set q \<times> {EPSend}"
-  by (auto simp: ep_q_refs_of'_def)
-
-lemma ntfn_q_refs_of'_simps[simp]:
- "ntfn_q_refs_of'  IdleNtfn         = {}"
- "ntfn_q_refs_of' (WaitingNtfn q)      = set q \<times> {NTFNSignal}"
- "ntfn_q_refs_of' (ActiveNtfn b)  = {}"
-  by (auto simp: ntfn_q_refs_of'_def)
+lemmas refs_of'_simps[simp] = refs_of'_def[split_simps kernel_object.split]
+lemmas tcb_st_refs_of'_simps[simp] = tcb_st_refs_of'_def[split_simps thread_state.split]
+lemmas ep_q_refs_of'_simps[simp] = ep_q_refs_of'_def[split_simps endpoint.split]
+lemmas ntfn_q_refs_of'_simps[simp] = ntfn_q_refs_of'_def[split_simps ntfn.split]
 
 lemma ntfn_bound_refs'_simps[simp]:
   "ntfn_bound_refs' (Some t) = {(t, NTFNBound)}"
@@ -1270,38 +1494,61 @@ lemma ntfn_bound_refs'_simps[simp]:
   by (auto simp: ntfn_bound_refs'_def)
 
 lemma tcb_bound_refs'_simps[simp]:
-  "tcb_bound_refs' (Some a) = {(a, TCBBound)}"
-  "tcb_bound_refs' None = {}"
+  "tcb_bound_refs' (Some a) b c = {(a, TCBBound)} \<union> tcb_bound_refs' None b c"
+  "tcb_bound_refs' b (Some a) c = {(a, TCBSchedContext)} \<union> tcb_bound_refs' b None c"
+  "tcb_bound_refs' b c (Some a) = {(a, TCBYieldTo)} \<union> tcb_bound_refs' b c None"
+  "tcb_bound_refs' None None None = {}"
   by (auto simp: tcb_bound_refs'_def)
 
+\<comment>\<open> Useful rewrite rules for extracting the existence of objects on the other side of symmetric refs.
+   There should be a rewrite corresponding to each entry of @{term symreftype}.\<close>
 lemma refs_of_rev':
- "(x, TCBBlockedRecv) \<in> refs_of' ko =
-    (\<exists>tcb. ko = KOTCB tcb \<and> (\<exists>a. tcbState tcb = BlockedOnReceive x a))"
- "(x, TCBBlockedSend) \<in> refs_of' ko =
+  "(x, TCBBlockedSend) \<in> refs_of' ko =
     (\<exists>tcb. ko = KOTCB tcb \<and> (\<exists>a b c d. tcbState tcb = BlockedOnSend x a b c d))"
- "(x, TCBSignal) \<in> refs_of' ko =
+  "(x, TCBBlockedRecv) \<in> refs_of' ko =
+    (\<exists>tcb. ko = KOTCB tcb \<and> (\<exists>a b. tcbState tcb = BlockedOnReceive x a b))"
+  "(x, TCBSignal) \<in> refs_of' ko =
     (\<exists>tcb. ko = KOTCB tcb \<and> tcbState tcb = BlockedOnNotification x)"
- "(x, EPRecv) \<in> refs_of' ko =
-    (\<exists>ep. ko = KOEndpoint ep \<and> (\<exists>q. ep = RecvEP q \<and> x \<in> set q))"
- "(x, EPSend) \<in> refs_of' ko =
-    (\<exists>ep. ko = KOEndpoint ep \<and> (\<exists>q. ep = SendEP q \<and> x \<in> set q))"
- "(x, NTFNSignal) \<in> refs_of' ko =
-    (\<exists>ntfn. ko = KONotification ntfn \<and> (\<exists>q. ntfnObj ntfn = WaitingNtfn q \<and> x \<in> set q))"
- "(x, TCBBound) \<in>  refs_of' ko =
+  "(x, TCBBound) \<in>  refs_of' ko =
     (\<exists>tcb. ko = KOTCB tcb \<and> (tcbBoundNotification tcb = Some x))"
- "(x, NTFNBound) \<in> refs_of' ko =
+  "(x, EPSend) \<in> refs_of' ko =
+    (\<exists>ep. ko = KOEndpoint ep \<and> (\<exists>q. ep = SendEP q \<and> x \<in> set q))"
+  "(x, EPRecv) \<in> refs_of' ko =
+    (\<exists>ep. ko = KOEndpoint ep \<and> (\<exists>q. ep = RecvEP q \<and> x \<in> set q))"
+  "(x, NTFNSignal) \<in> refs_of' ko =
+    (\<exists>ntfn. ko = KONotification ntfn \<and> (\<exists>q. ntfnObj ntfn = WaitingNtfn q \<and> x \<in> set q))"
+  "(x, NTFNBound) \<in> refs_of' ko =
     (\<exists>ntfn. ko = KONotification ntfn \<and> (ntfnBoundTCB ntfn = Some x))"
+  "(x, TCBSchedContext) \<in> refs_of' ko =
+    (\<exists>tcb. ko = KOTCB tcb \<and> tcbSchedContext tcb = Some x)"
+  "(x, SCTcb) \<in> refs_of' ko =
+    (\<exists>sc. ko = KOSchedContext sc \<and> scTCB sc = Some x)"
+  "(x, NTFNSchedContext) \<in> refs_of' ko =
+    (\<exists>ntfn. ko = KONotification ntfn \<and> ntfnSc ntfn = Some x)"
+  "(x, SCNtfn) \<in> refs_of' ko =
+    (\<exists>sc. ko = KOSchedContext sc \<and> scNtfn sc = Some x)"
+  "(x, SCReply) \<in> refs_of' ko =
+    (\<exists>sc. ko = KOSchedContext sc \<and> scReply sc = Some x)"
+  "(x, ReplySchedContext) \<in> refs_of' ko =
+    (\<exists>reply. ko = KOReply reply \<and> replySC reply = Some x)"
+  "(x, ReplyTCB) \<in> refs_of' ko =
+    (\<exists>reply. ko = KOReply reply \<and> replyTCB reply = Some x)"
+  "(x, TCBYieldTo) \<in> refs_of' ko =
+    (\<exists>tcb. ko = KOTCB tcb \<and> tcbYieldTo tcb = Some x)"
+  "(x, SCYieldFrom) \<in> refs_of' ko =
+    (\<exists>sc. ko = KOSchedContext sc \<and> scYieldFrom sc = Some x)"
   by (auto simp: refs_of'_def
                  tcb_st_refs_of'_def
                  ep_q_refs_of'_def
                  ntfn_q_refs_of'_def
                  ntfn_bound_refs'_def
                  tcb_bound_refs'_def
+                 in_get_refs
           split: Structures_H.kernel_object.splits
                  Structures_H.thread_state.splits
                  Structures_H.endpoint.splits
                  Structures_H.notification.splits
-                 Structures_H.ntfn.splits)+
+                 Structures_H.ntfn.splits)
 
 lemma ko_wp_at'_weakenE:
   "\<lbrakk> ko_wp_at' P p s; \<And>ko. P ko \<Longrightarrow> Q ko \<rbrakk> \<Longrightarrow> ko_wp_at' Q p s"
@@ -1313,7 +1560,7 @@ lemma projectKO_opt_tcbD:
 
 lemma st_tcb_at_refs_of_rev':
   "ko_wp_at' (\<lambda>ko. (x, TCBBlockedRecv) \<in> refs_of' ko) t s
-     = st_tcb_at' (\<lambda>ts. \<exists>a. ts = BlockedOnReceive x a) t s"
+     = st_tcb_at' (\<lambda>ts. \<exists>a b. ts = BlockedOnReceive x a b) t s"
   "ko_wp_at' (\<lambda>ko. (x, TCBBlockedSend) \<in> refs_of' ko) t s
      = st_tcb_at' (\<lambda>ts. \<exists>a b c d. ts = BlockedOnSend x a b c d) t s"
   "ko_wp_at' (\<lambda>ko. (x, TCBSignal) \<in> refs_of' ko) t s
@@ -1345,14 +1592,23 @@ where
   "tcb_ntfn_is_bound' ntfn tcb \<equiv> tcbBoundNotification tcb = ntfn"
 
 lemma st_tcb_at_state_refs_ofD':
-  "st_tcb_at' P t s \<Longrightarrow> \<exists>ts ntfnptr. P ts \<and> obj_at' (tcb_ntfn_is_bound' ntfnptr) t s
-          \<and> state_refs_of' s t = (tcb_st_refs_of' ts \<union> tcb_bound_refs' ntfnptr)"
+  "st_tcb_at' P t s \<Longrightarrow>
+    \<exists>ts ntfnptr sc_ptr yieldto_ptr. P ts
+                 \<and> obj_at' ((=) ntfnptr o tcbBoundNotification) t s
+                 \<and> obj_at' ((=) sc_ptr o tcbSchedContext) t s
+                 \<and> obj_at' ((=) yieldto_ptr o tcbYieldTo) t s
+                 \<and> state_refs_of' s t = (tcb_st_refs_of' ts
+                                         \<union> tcb_bound_refs' ntfnptr sc_ptr yieldto_ptr)"
   by (auto simp: pred_tcb_at'_def tcb_ntfn_is_bound'_def obj_at'_def projectKO_eq
                  project_inject state_refs_of'_def)
 
 lemma bound_tcb_at_state_refs_ofD':
-  "bound_tcb_at' P t s \<Longrightarrow> \<exists>ts ntfnptr. P ntfnptr \<and> obj_at' (tcb_ntfn_is_bound' ntfnptr) t s
-          \<and> state_refs_of' s t = (tcb_st_refs_of' ts \<union> tcb_bound_refs' ntfnptr)"
+  "bound_tcb_at' P t s \<Longrightarrow>
+    \<exists>ts ntfnptr sc_ptr yieldto_ptr. P ntfnptr
+                 \<and> obj_at' ((=) ntfnptr o tcbBoundNotification) t s
+                 \<and> obj_at' ((=) sc_ptr o tcbSchedContext) t s
+                 \<and> obj_at' ((=) yieldto_ptr o tcbYieldTo) t s
+          \<and> state_refs_of' s t = (tcb_st_refs_of' ts \<union> tcb_bound_refs' ntfnptr sc_ptr yieldto_ptr)"
   by (auto simp: pred_tcb_at'_def obj_at'_def tcb_ntfn_is_bound'_def projectKO_eq
                  project_inject state_refs_of'_def)
 
@@ -1375,13 +1631,17 @@ lemma sym_refs_ko_atD':
 
 lemma sym_refs_st_tcb_atD':
   "\<lbrakk> st_tcb_at' P t s; sym_refs (state_refs_of' s) \<rbrakk> \<Longrightarrow>
-     \<exists>ts ntfnptr. P ts \<and> obj_at' (tcb_ntfn_is_bound' ntfnptr) t s
-        \<and> state_refs_of' s t = tcb_st_refs_of' ts \<union> tcb_bound_refs' ntfnptr
-        \<and> (\<forall>(x, tp)\<in>tcb_st_refs_of' ts \<union> tcb_bound_refs' ntfnptr. ko_wp_at' (\<lambda>ko. (t, symreftype tp) \<in> refs_of' ko) x s)"
+     \<exists>ts ntfnptr sc_ptr yieldto_ptr. P ts
+        \<and> obj_at' ((=) ntfnptr o tcbBoundNotification) t s
+        \<and> state_refs_of' s t = tcb_st_refs_of' ts \<union> tcb_bound_refs' ntfnptr sc_ptr yieldto_ptr
+        \<and> (\<forall>(x, tp)\<in>tcb_st_refs_of' ts \<union> tcb_bound_refs' ntfnptr sc_ptr yieldto_ptr.
+              ko_wp_at' (\<lambda>ko. (t, symreftype tp) \<in> refs_of' ko) x s)"
   apply (drule st_tcb_at_state_refs_ofD')
   apply (erule exE)+
   apply (rule_tac x=ts in exI)
   apply (rule_tac x=ntfnptr in exI)
+  apply (rule_tac x=sc_ptr in exI)
+  apply (rule_tac x=yieldto_ptr in exI)
   apply clarsimp
   apply (frule obj_at_state_refs_ofD')
   apply (drule (1)sym_refs_obj_atD')
@@ -1390,26 +1650,46 @@ lemma sym_refs_st_tcb_atD':
 
 lemma sym_refs_bound_tcb_atD':
   "\<lbrakk> bound_tcb_at' P t s; sym_refs (state_refs_of' s) \<rbrakk> \<Longrightarrow>
-     \<exists>ts ntfnptr. P ntfnptr \<and> obj_at' (tcb_ntfn_is_bound' ntfnptr) t s
-        \<and> state_refs_of' s t = tcb_st_refs_of' ts \<union> tcb_bound_refs' ntfnptr
-        \<and> (\<forall>(x, tp)\<in>tcb_st_refs_of' ts \<union> tcb_bound_refs' ntfnptr. ko_wp_at' (\<lambda>ko. (t, symreftype tp) \<in> refs_of' ko) x s)"
+     \<exists>ts ntfnptr sc_ptr yieldto_ptr. P ntfnptr
+        \<and> obj_at' ((=) ntfnptr o tcbBoundNotification) t s
+        \<and> state_refs_of' s t = tcb_st_refs_of' ts \<union> tcb_bound_refs' ntfnptr sc_ptr yieldto_ptr
+        \<and> (\<forall>(x, tp)\<in>tcb_st_refs_of' ts \<union> tcb_bound_refs' ntfnptr sc_ptr yieldto_ptr.
+              ko_wp_at' (\<lambda>ko. (t, symreftype tp) \<in> refs_of' ko) x s)"
   apply (drule bound_tcb_at_state_refs_ofD')
   apply (erule exE)+
   apply (rule_tac x=ts in exI)
   apply (rule_tac x=ntfnptr in exI)
+  apply (rule_tac x=sc_ptr in exI)
+  apply (rule_tac x=yieldto_ptr in exI)
   apply clarsimp
   apply (frule obj_at_state_refs_ofD')
   apply (drule (1)sym_refs_obj_atD')
   apply auto
   done
 
-lemma refs_of_live':
-  "refs_of' ko \<noteq> {} \<Longrightarrow> live' ko"
-  apply (cases ko, simp_all)
-    apply clarsimp
-   apply (rename_tac notification)
-   apply (case_tac "ntfnObj notification"; simp)
-    apply fastforce+
+lemma get_refs_nonempty[simp]:
+  "(get_refs ref_ty ptr_opt \<noteq> {}) = (ptr_opt \<noteq> None)"
+  by (clarsimp simp: get_refs_def split: option.splits)
+
+lemma get_refs_empty[simp]:
+  "(get_refs ref_ty ptr_opt = {}) = (ptr_opt = None)"
+  by (clarsimp simp: get_refs_def split: option.splits)
+
+abbreviation idle_refs :: "(machine_word \<times> reftype) set" where
+  "idle_refs \<equiv> {(idle_sc_ptr, TCBSchedContext), (idle_thread_ptr, SCTcb)}"
+
+\<comment>\<open> This set subtraction gets simplified into a subset relation at all the places
+    we might want to use this rule, so we do that ahead of time. \<close>
+lemma refs_of_live'[simplified]:
+  "refs_of' ko - idle_refs \<noteq> {} \<Longrightarrow> live' ko"
+  apply (cases ko; simp)
+      apply clarsimp
+     apply (rename_tac notification)
+     apply (case_tac "ntfnObj notification";
+            fastforce simp: live_ntfn'_def)
+    apply fastforce
+   apply (fastforce simp: live_sc'_def)
+  apply (fastforce simp: live_reply'_def)
   done
 
 lemma if_live_then_nonz_capE':
@@ -1426,10 +1706,11 @@ lemma if_live_then_nonz_capD':
 
 lemma if_live_state_refsE:
   "\<lbrakk> if_live_then_nonz_cap' s;
-     state_refs_of' s p \<noteq> {} \<rbrakk> \<Longrightarrow> ex_nonz_cap_to' p s"
-  by (clarsimp simp: state_refs_of'_def ko_wp_at'_def
-              split: option.splits if_split_asm
-              elim!: refs_of_live' if_live_then_nonz_capE')
+     state_refs_of' s p - idle_refs \<noteq> {} \<rbrakk> \<Longrightarrow> ex_nonz_cap_to' p s"
+  apply (erule if_live_then_nonz_capE')
+  apply (simp add: state_refs_of'_def ko_wp_at'_def refs_of_live'
+              split: if_split_asm option.splits)
+  done
 
 lemmas ex_cte_cap_to'_def = ex_cte_cap_wp_to'_def
 
@@ -1453,6 +1734,10 @@ lemma valid_objsE' [elim]:
   "\<lbrakk> valid_objs' s; ksPSpace s x = Some obj; valid_obj' obj s \<Longrightarrow> R \<rbrakk> \<Longrightarrow> R"
   unfolding valid_objs'_def by auto
 
+lemma valid_objs_sizeE' [elim]:
+  "\<lbrakk> valid_objs_size' s; ksPSpace s x = Some obj; valid_obj_size' obj s \<Longrightarrow> R \<rbrakk> \<Longrightarrow> R"
+  unfolding valid_objs_size'_def by auto
+
 lemma pspace_distinctD':
   "\<lbrakk> ksPSpace s x = Some v; pspace_distinct' s \<rbrakk> \<Longrightarrow> ps_clear x (objBitsKO v) s"
   apply (simp add: pspace_distinct'_def)
@@ -1467,30 +1752,33 @@ lemma pspace_alignedD':
   apply simp
   done
 
+lemma pspace_boundedD':
+  "\<lbrakk> ksPSpace s x = Some v; pspace_bounded' s \<rbrakk> \<Longrightarrow> objBitsKO v < word_bits"
+  apply (simp add: pspace_bounded'_def)
+  apply (drule bspec, erule domI)
+  apply simp
+  done
+
 lemma next_unfold:
   "mdb_next s c =
    (case s c of Some cte \<Rightarrow> Some (mdbNext (cteMDBNode cte)) | None \<Rightarrow> None)"
   by (simp add: mdb_next_def split: option.split)
 
-lemma is_physical_cases:
- "(capClass cap = PhysicalClass) =
-  (case cap of NullCap                         \<Rightarrow> False
-             | DomainCap                       \<Rightarrow> False
-             | IRQControlCap                   \<Rightarrow> False
-             | IRQHandlerCap irq               \<Rightarrow> False
-             | ReplyCap r m cr                 \<Rightarrow> False
-             | ArchObjectCap ASIDControlCap    \<Rightarrow> False
-             | _                               \<Rightarrow> True)"
-  by (simp split: capability.splits arch_capability.splits zombie_type.splits)
-
 lemma sch_act_sane_not:
   "sch_act_sane s = sch_act_not (ksCurThread s) s"
   by (auto simp: sch_act_sane_def)
 
-lemma objBits_cte_conv: "objBits (cte :: cte) = cteSizeBits"
+lemma objBits_cte_conv:
+  "objBits (cte :: cte) = cteSizeBits"
   by (simp add: objBits_simps word_size)
 
 lemmas valid_irq_states'_def = valid_irq_masks'_def
+
+lemma valid_pspaceI' [intro]:
+  "\<lbrakk>valid_objs' s; pspace_aligned' s; pspace_distinct' s; pspace_bounded' s; valid_mdb' s; no_0_obj' s;
+    valid_replies' s; pspace_canonical' s; pspace_in_kernel_mappings' s\<rbrakk>
+  \<Longrightarrow> valid_pspace' s"
+  unfolding valid_pspace'_def by simp
 
 lemma valid_pspaceE' [elim]:
   "\<lbrakk>valid_pspace' s;
@@ -1498,23 +1786,22 @@ lemma valid_pspaceE' [elim]:
       valid_mdb' s; pspace_canonical' s; pspace_in_kernel_mappings' s\<rbrakk> \<Longrightarrow> R \<rbrakk> \<Longrightarrow> R"
   unfolding valid_pspace'_def by simp
 
-lemma idle'_no_refs:
-  "valid_idle' s \<Longrightarrow> state_refs_of' s (ksIdleThread s) = {}"
+lemma idle'_only_sc_refs:
+  "valid_idle' s \<Longrightarrow> state_refs_of' s (ksIdleThread s) = {(idle_sc_ptr, TCBSchedContext)}"
   by (clarsimp simp: valid_idle'_def pred_tcb_at'_def obj_at'_def tcb_ntfn_is_bound'_def
                      projectKO_eq project_inject state_refs_of'_def idle_tcb'_def)
 
 lemma idle'_not_queued':
   "\<lbrakk>valid_idle' s; sym_refs (state_refs_of' s);
-    state_refs_of' s ptr = insert t queue \<times> {rt}\<rbrakk>\<Longrightarrow>
-   ksIdleThread s \<notin> queue"
-  by (frule idle'_no_refs, fastforce simp: valid_idle'_def sym_refs_def)
+    state_refs_of' s ptr = insert t queue \<times> {rt}; ksIdleThread s \<in> queue\<rbrakk>
+     \<Longrightarrow> ptr = idle_sc_ptr"
+  by (frule idle'_only_sc_refs, fastforce simp: valid_idle'_def sym_refs_def)
 
 lemma idle'_not_queued:
   "\<lbrakk>valid_idle' s; sym_refs (state_refs_of' s);
-    state_refs_of' s ptr = queue \<times> {rt}\<rbrakk> \<Longrightarrow>
-   ksIdleThread s \<notin> queue"
-  by (frule idle'_no_refs, fastforce simp: valid_idle'_def sym_refs_def)
-
+    state_refs_of' s ptr = queue \<times> {rt}; ksIdleThread s \<in> queue\<rbrakk>
+      \<Longrightarrow> ptr = idle_sc_ptr"
+  by (frule idle'_only_sc_refs, fastforce simp: valid_idle'_def sym_refs_def)
 
 lemma obj_at_conj':
   "\<lbrakk> obj_at' P p s; obj_at' Q p s \<rbrakk> \<Longrightarrow> obj_at' (\<lambda>k. P k \<and> Q k) p s"
@@ -1525,6 +1812,10 @@ lemma pred_tcb_at_conj':
   apply (simp add: pred_tcb_at'_def)
   apply (erule (1) obj_at_conj')
   done
+
+lemma pred_tcb_at'_eq_commute:
+  "pred_tcb_at' proj ((=) v) = pred_tcb_at' proj (\<lambda>x. x = v)"
+  by (intro ext) (auto simp: pred_tcb_at'_def obj_at'_def)
 
 lemma obj_at_False' [simp]:
   "obj_at' (\<lambda>k. False) t s = False"
@@ -1538,23 +1829,29 @@ lemma obj_at'_pspaceI:
   "obj_at' t ref s \<Longrightarrow> ksPSpace s = ksPSpace s' \<Longrightarrow>  obj_at' t ref s'"
   by (auto intro!: projectKO_stateI simp: obj_at'_def ps_clear_def)
 
+lemma sc_at'_n_pspaceI:
+  "sc_at'_n n ref s \<Longrightarrow> ksPSpace s = ksPSpace s' \<Longrightarrow>  sc_at'_n n ref s'"
+  by (auto intro!: projectKO_stateI simp: ko_wp_at'_def ps_clear_def)
+
 lemma cte_wp_at'_pspaceI:
   "\<lbrakk>cte_wp_at' P p s; ksPSpace s = ksPSpace s'\<rbrakk> \<Longrightarrow> cte_wp_at' P p s'"
-  apply (clarsimp simp add: cte_wp_at'_def getObject_def)
+  supply if_cong[cong]
+  apply (clarsimp simp: cte_wp_at'_def getObject_def readObject_def gets_the_def)
   apply (drule equalityD2)
-  apply (clarsimp simp: in_monad loadObject_cte gets_def
-                        get_def bind_def return_def split_def)
-  apply (case_tac b)
-        apply (simp_all add: in_monad typeError_def)
+  apply (clarsimp simp: in_monad loadObject_cte gets_def asks_def
+                        get_def bind_def split_def oassert_opt_def
+                 split: option.split_asm)
+  apply (rename_tac b; case_tac b)
+           apply (simp_all add: in_monad read_typeError_def)
    prefer 2
-   apply (simp add: in_monad return_def alignError_def assert_opt_def
-                    alignCheck_def magnitudeCheck_def when_def bind_def
+   apply (simp add: in_monad omonad_defs read_alignError_def obind_def
+                    read_alignCheck_def read_magnitudeCheck_def return_def
              split: if_split_asm option.splits)
-  apply (clarsimp simp: in_monad return_def alignError_def fail_def assert_opt_def
-                        alignCheck_def bind_def when_def
+  apply (clarsimp simp: in_monad omonad_defs read_alignError_def obind_def
+                        read_alignCheck_def read_magnitudeCheck_def return_def
                         objBits_cte_conv tcbCTableSlot_def tcbVTableSlot_def
-                        tcbReplySlot_def objBits_defs
-                 split: if_split_asm cong: image_cong
+                        cteSizeBits_def tcbIPCBufferSlot_def tcbFaultHandlerSlot_def
+                 split: if_split_asm option.split_asm
                  dest!: singleton_in_magnitude_check)
   done
 
@@ -1577,21 +1874,24 @@ lemma valid_cap'_pspaceI:
   by (cases cap)
      (auto intro: obj_at'_pspaceI[rotated]
                   cte_wp_at'_pspaceI valid_untyped'_pspaceI
-                  typ_at'_pspaceI[rotated] frame_at'_pspaceI[rotated]
+                  typ_at'_pspaceI[rotated] sc_at'_n_pspaceI[rotated] frame_at'_pspaceI[rotated]
             simp: vspace_table_at'_defs valid_arch_cap'_def valid_arch_cap_ref'_def
            split: arch_capability.split zombie_type.split option.splits)
-
 
 lemma valid_obj'_pspaceI:
   "valid_obj' obj s \<Longrightarrow> ksPSpace s = ksPSpace s' \<Longrightarrow> valid_obj' obj s'"
   unfolding valid_obj'_def
   by (cases obj)
      (auto simp: valid_ep'_def valid_ntfn'_def valid_tcb'_def valid_cte'_def
-                 valid_tcb_state'_def valid_bound_tcb'_def
-                 valid_bound_ntfn'_def
+                 valid_tcb_state'_def valid_bound_obj'_def valid_sched_context'_def valid_reply'_def
            split: Structures_H.endpoint.splits Structures_H.notification.splits
                   Structures_H.thread_state.splits ntfn.splits option.splits
            intro: obj_at'_pspaceI valid_cap'_pspaceI)
+
+lemma valid_obj_size'_pspaceI:
+  "valid_obj_size' obj s \<Longrightarrow> ksPSpace s = ksPSpace s' \<Longrightarrow> valid_obj_size' obj s'"
+  unfolding valid_obj_size'_def
+  by (cases obj; simp)
 
 lemma pred_tcb_at'_pspaceI:
   "pred_tcb_at' proj P t s \<Longrightarrow> ksPSpace s = ksPSpace s' \<Longrightarrow> pred_tcb_at' proj P t s'"
@@ -1601,16 +1901,24 @@ lemma valid_mdb'_pspaceI:
   "valid_mdb' s \<Longrightarrow> ksPSpace s = ksPSpace s' \<Longrightarrow> valid_mdb' s'"
   unfolding valid_mdb'_def by simp
 
+lemma valid_replies'_pspaceI:
+  "valid_replies' s \<Longrightarrow> ksPSpace s = ksPSpace s' \<Longrightarrow> valid_replies' s'"
+  unfolding valid_replies'_def
+  apply clarsimp
+  apply (drule_tac x=rptr in spec)
+  apply (auto simp: opt_map_def intro: pred_tcb_at'_pspaceI)
+  done
+
 lemma state_refs_of'_pspaceI:
   "P (state_refs_of' s) \<Longrightarrow> ksPSpace s = ksPSpace s' \<Longrightarrow> P (state_refs_of' s')"
   unfolding state_refs_of'_def ps_clear_def by (simp cong: option.case_cong)
 
 lemma valid_pspace':
   "valid_pspace' s \<Longrightarrow> ksPSpace s = ksPSpace s' \<Longrightarrow> valid_pspace' s'"
-  by  (auto simp add: valid_pspace'_def valid_objs'_def pspace_aligned'_def pspace_canonical'_def
-                     pspace_distinct'_def ps_clear_def no_0_obj'_def ko_wp_at'_def
-                     typ_at'_def pspace_in_kernel_mappings'_def
-           intro: valid_obj'_pspaceI valid_mdb'_pspaceI)
+  by  (auto simp: valid_pspace'_def valid_objs'_def pspace_aligned'_def pspace_canonical'_def
+                  pspace_distinct'_def ps_clear_def no_0_obj'_def ko_wp_at'_def
+                  typ_at'_def pspace_in_kernel_mappings'_def pspace_bounded'_def
+           intro: valid_obj'_pspaceI valid_mdb'_pspaceI valid_replies'_pspaceI)
 
 lemma ex_cte_cap_to_pspaceI'[elim]:
   "ex_cte_cap_to' p s \<Longrightarrow> ksPSpace s = ksPSpace s' \<Longrightarrow>
@@ -1622,8 +1930,9 @@ lemma valid_idle'_pspace_itI[elim]:
   "\<lbrakk> valid_idle' s; ksPSpace s = ksPSpace s'; ksIdleThread s = ksIdleThread s' \<rbrakk>
       \<Longrightarrow> valid_idle' s'"
   apply (clarsimp simp: valid_idle'_def ex_nonz_cap_to'_def)
-  apply (erule obj_at'_pspaceI, assumption)
-  done
+  apply (rule conjI)
+   apply (erule obj_at'_pspaceI, assumption)
+  using obj_at'_pspaceI by blast
 
 lemma obj_at'_weaken:
   assumes x: "obj_at' P t s"
@@ -1782,43 +2091,82 @@ lemma ps_clear_lookupAround2:
   apply (drule word_le_minus_one_leq, fastforce)
   done
 
-lemma in_magnitude_check:
-  "\<lbrakk> is_aligned x n; (1 :: machine_word) < 2 ^ n; ksPSpace s x = Some y \<rbrakk> \<Longrightarrow>
-   ((v, s') \<in> fst (magnitudeCheck x (snd (lookupAround2 x (ksPSpace s))) n s))
-     = (s' = s \<and> ps_clear x n s)"
-  apply (rule iffI)
-   apply (clarsimp simp: magnitudeCheck_def in_monad lookupAround2_None2
-                         lookupAround2_char2
-                  split: option.split_asm)
-    apply (erule(1) ps_clearI)
-    apply simp
-   apply (erule(1) ps_clearI)
-   apply (simp add: linorder_not_less)
-   apply (drule word_leq_le_minus_one[where x="2 ^ n"])
-    apply (clarsimp simp: power_overflow)
-   apply (drule word_l_diffs)
-    apply simp
-   apply (simp add: field_simps)
-  apply clarsimp
-  apply (erule is_aligned_get_word_bits)
-   apply (erule(1) ps_clear_lookupAround2)
-     apply simp
-    apply (simp add: is_aligned_no_overflow)
-   apply (clarsimp simp add: magnitudeCheck_def in_monad
-                      split: option.split_asm)
-   apply simp
-  apply (simp add: power_overflow)
+lemma magnitudeCheck_wp:
+  "\<lbrace>\<lambda>s. (case next of
+                  Some next' \<Rightarrow> next' - ptr \<ge> 1 << bits
+                | None \<Rightarrow> True)
+        \<longrightarrow> P s\<rbrace>
+   magnitudeCheck ptr next bits
+   \<lbrace>\<lambda>_. P\<rbrace>"
+  unfolding magnitudeCheck_def read_magnitudeCheck_def
+  apply (simp add: gets_the_def exec_gets assert_opt_def valid_def
+                   return_def split_def fail_def
+            split: option.split)
   done
 
-lemma in_magnitude_check3:
+lemma alignCheck_wp:
+  "\<lbrace>\<lambda>s. is_aligned ptr bits \<longrightarrow> P s\<rbrace>
+   alignCheck ptr bits
+   \<lbrace>\<lambda>_. P\<rbrace>"
+  unfolding alignCheck_def read_alignCheck_def
+  apply (wpsimp simp: read_alignError_def is_aligned_mask omonad_defs)
+  done
+
+lemma lookupAround2_no_after_ps_clear:
+  "snd (lookupAround2 p (ksPSpace s)) = None \<Longrightarrow> ps_clear p bits s"
+  apply (fastforce simp: ps_clear_def lookupAround2_None2 dom_def set_eq_iff word_le_less_eq)
+  done
+
+lemma lookupAround2_after_ps_clear:
+  "\<lbrakk>snd (lookupAround2 p (ksPSpace s)) = Some after;
+    2 ^ bits \<le> after - p;
+    1 < (2 :: machine_word) ^ bits;
+    is_aligned p bits\<rbrakk> \<Longrightarrow>
+   ps_clear p bits s"
+  apply (rule ps_clearI; clarsimp simp: lookupAround2_char2)
+  apply (rename_tac x obj_after)
+  apply (drule_tac x=x in spec)
+  apply (frule word_l_diffs, simp)
+  apply (prop_tac "x < after")
+   apply (frule word_leq_minus_one_le[rotated])
+    apply (metis add.commute arith_simps(49) plus_minus_not_NULL_ab word_le_less_eq
+                 word_not_simps(1))
+   apply (frule_tac a=x in order.strict_trans2; fastforce simp: add.commute)
+  apply clarsimp
+  done
+
+lemma read_magnitude_check_simp[simp]:
+  assumes "is_aligned ptr bits"
+          "(1 :: machine_word) < 2 ^ bits"
+          "ksPSpace s ptr = Some y"
+  shows "read_magnitudeCheck ptr (snd (lookupAround2 ptr (ksPSpace s))) bits s = Some ()
+          = ps_clear ptr bits s"
+  using assms
+  apply (clarsimp simp: read_magnitudeCheck_def)
+  apply (rule iffI)
+   apply (clarsimp simp: lookupAround2_no_after_ps_clear lookupAround2_after_ps_clear omonad_defs
+                  split: option.splits if_split_asm)
+  apply (fastforce elim!: ps_clear_lookupAround2 is_aligned_no_overflow split: option.splits)
+  done
+
+lemma in_magnitude_check:
+  assumes "is_aligned ptr bits"
+          "(1 :: machine_word) < 2 ^ bits"
+          "ksPSpace s ptr = Some y"
+  shows "((v, s') \<in> fst (magnitudeCheck ptr (snd (lookupAround2 ptr (ksPSpace s))) bits s))
+          = (s' = s \<and> ps_clear ptr bits s)"
+  using assms
+  by (clarsimp simp: magnitudeCheck_def in_monad)
+
+lemma read_magnitude_check3[simp]:
   "\<lbrakk> \<forall>z. x < z \<and> z \<le> y \<longrightarrow> ksPSpace s z = None; is_aligned x n;
      (1 :: machine_word) < 2 ^ n; ksPSpace s x = Some v; x \<le> y; y - x < 2 ^ n \<rbrakk> \<Longrightarrow>
-   fst (magnitudeCheck x (snd (lookupAround2 y (ksPSpace s))) n s)
-     = (if ps_clear x n s then {((), s)} else {})"
-  apply (rule set_eqI, rule iffI)
-   apply (clarsimp simp: magnitudeCheck_def lookupAround2_char2
-                         lookupAround2_None2 in_monad
-                  split: option.split_asm)
+   read_magnitudeCheck x (snd (lookupAround2 y (ksPSpace s))) n s
+     = (if ps_clear x n s then Some () else None)"
+  apply (clarsimp simp: read_magnitudeCheck_def lookupAround2_char2
+                        lookupAround2_None2 in_monad
+                 split: option.splits)
+  apply safe
     apply (drule(1) range_convergence1)
     apply (erule(1) ps_clearI)
     apply simp
@@ -1830,7 +2178,6 @@ lemma in_magnitude_check3:
     apply (drule word_l_diffs, simp)
     apply (simp add: field_simps)
    apply (simp add: power_overflow)
-  apply (clarsimp split: if_split_asm)
   apply (erule(1) ps_clear_lookupAround2)
     apply simp
    apply (drule word_le_minus_one_leq[where x="y - x"])
@@ -1839,16 +2186,28 @@ lemma in_magnitude_check3:
      apply (simp add: field_simps is_aligned_no_overflow)
     apply simp
    apply (simp add: field_simps)
-  apply (simp add: magnitudeCheck_def return_def
-                   iffD2[OF linorder_not_less] when_def
-            split: option.split_asm)
+  apply (fastforce simp: lookupAround2_None2 lookupAround2_char2
+                  split: option.split_asm)
   done
+
+lemma in_magnitude_check3:
+  "\<lbrakk> \<forall>z. x < z \<and> z \<le> y \<longrightarrow> ksPSpace s z = None; is_aligned x n;
+     (1 :: machine_word) < 2 ^ n; ksPSpace s x = Some v; x \<le> y; y - x < 2 ^ n \<rbrakk> \<Longrightarrow>
+   fst (magnitudeCheck x (snd (lookupAround2 y (ksPSpace s))) n s)
+     = (if ps_clear x n s then {((), s)} else {})"
+  apply (clarsimp simp: magnitudeCheck_def gets_the_def
+                        exec_gets in_monad return_def assert_opt_def fail_def
+                 split: option.split_asm)
+  done
+
+lemma read_alignCheck_simp[simp]:
+  "read_alignCheck x n s = Some v = is_aligned x n"
+  by (simp add: read_alignCheck_def is_aligned_mask[symmetric]
+                read_alignError_def omonad_defs)
 
 lemma in_alignCheck[simp]:
   "((v, s') \<in> fst (alignCheck x n s)) = (s' = s \<and> is_aligned x n)"
-  by (simp add: alignCheck_def in_monad is_aligned_mask[symmetric]
-                alignError_def conj_comms
-          cong: conj_cong)
+  by (simp add: alignCheck_def in_monad)
 
 lemma tcb_space_clear:
   "\<lbrakk> tcb_cte_cases (y - x) = Some (getF, setF);
@@ -1891,32 +2250,28 @@ lemma cte_wp_at_cases':
              \<and> tcb_cte_cases n = Some (getF, setF) \<and> P (getF tcb) \<and> ps_clear (p - n) tcbBlockSizeBits s))"
   (is "?LHS = ?RHS")
   apply (rule iffI)
-   apply (clarsimp simp: cte_wp_at'_def split_def
-                         getObject_def bind_def simpler_gets_def
+   apply (clarsimp simp: cte_wp_at'_def gets_the_def readObject_def
+                         getObject_def bind_def simpler_gets_def omonad_defs
                          assert_opt_def return_def fail_def
-                  split: option.splits
+                  split: option.splits dest!: prod_injects
                     del: disjCI)
-   apply (clarsimp simp: loadObject_cte typeError_def alignError_def
+   apply (clarsimp simp: loadObject_cte read_typeError_def split_def
                          fail_def return_def objBits_simps'
-                         is_aligned_mask[symmetric] alignCheck_def
+                         is_aligned_mask[symmetric]
                          tcbVTableSlot_def field_simps tcbCTableSlot_def
-                         tcbReplySlot_def tcbCallerSlot_def
                          tcbIPCBufferSlot_def
-                         lookupAround2_char1
+                         tcbFaultHandlerSlot_def tcbTimeoutHandlerSlot_def
+                         lookupAround2_char1 omonad_defs
                          cte_level_bits_def Ball_def
-                         unless_def when_def bind_def
+                         unless_def when_def bind_def alignError_def alignCheck_def
                   split: kernel_object.splits if_split_asm option.splits
                     del: disjCI)
-        apply (subst(asm) in_magnitude_check3, simp+,
-               simp split: if_split_asm, (rule disjI2)?, intro exI, rule conjI,
-               erule rsubst[where P="\<lambda>x. ksPSpace s x = v" for s v],
-               fastforce simp add: field_simps, simp)+
-   apply (subst(asm) in_magnitude_check3, simp+)
-   apply (simp split: if_split_asm
-                add: )
+       apply (rule disjI2)
+       apply (fastforce simp: field_simps elim: rsubst[where P="\<lambda>x. ksPSpace s x = v" for s v])+
   apply (simp add: cte_wp_at'_def getObject_def split_def
                    bind_def simpler_gets_def return_def
                    assert_opt_def fail_def objBits_defs
+                   readObject_def omonad_defs obind_def gets_the_def
             split: option.splits)
   apply (elim disjE conjE exE)
    apply (erule(1) ps_clear_lookupAround2)
@@ -1928,7 +2283,9 @@ lemma cte_wp_at_cases':
    apply (simp add: loadObject_cte unless_def alignCheck_def
                     is_aligned_mask[symmetric] objBits_simps'
                     cte_level_bits_def magnitudeCheck_def
-                    return_def fail_def)
+                    return_def fail_def obind_def
+                    read_magnitudeCheck_def read_alignCheck_def
+                    omonad_defs)
    apply (clarsimp simp: bind_def return_def when_def fail_def
                   split: option.splits)
    apply simp
@@ -1938,7 +2295,8 @@ lemma cte_wp_at_cases':
                      is_aligned_mask[symmetric] objBits_simps'
                      cte_level_bits_def magnitudeCheck_def
                      return_def fail_def tcbCTableSlot_def tcbVTableSlot_def
-                     tcbIPCBufferSlot_def tcbReplySlot_def tcbCallerSlot_def
+                     tcbIPCBufferSlot_def tcbFaultHandlerSlot_def tcbTimeoutHandlerSlot_def
+                     omonad_defs obind_def read_magnitudeCheck_def read_alignCheck_def
               split: option.split_asm)
      apply (clarsimp simp: bind_def tcb_cte_cases_def cteSizeBits_def split: if_split_asm)
     apply (clarsimp simp: bind_def tcb_cte_cases_def iffD2[OF linorder_not_less]
@@ -1958,7 +2316,7 @@ lemma cte_wp_at_cases':
 
 lemma tcb_at_cte_at':
   "tcb_at' t s \<Longrightarrow> cte_at' t s"
-  apply (clarsimp simp add: cte_wp_at_cases' obj_at'_def projectKO_def
+  apply (clarsimp simp add: cte_wp_at_cases' obj_at'_def projectKO_def oassert_opt_def
                        del: disjCI)
   apply (case_tac ko)
    apply (simp_all add: projectKO_opt_tcb fail_def)
@@ -2002,14 +2360,30 @@ lemma obj_at_ko_at':
   "obj_at' P p s \<Longrightarrow> \<exists>ko. ko_at' ko p s \<and> P ko"
   by (auto simp add: obj_at'_def)
 
+lemma ko_at_obj_at':
+  "\<lbrakk>ko_at' ko ptr s; P ko\<rbrakk> \<Longrightarrow>
+   obj_at' P ptr s"
+  by (clarsimp simp: obj_at'_def)
+
+lemma obj_at_ko_at'_eq:
+  "(\<exists>ko. ko_at' ko p s \<and> P ko) = obj_at' P p s"
+  apply (intro iffI; clarsimp simp: obj_at_ko_at')
+  unfolding obj_at'_def
+  by blast
+
+lemma ko_at'_replies_of':
+  "ko_at' reply ptr s \<Longrightarrow> replies_of' s ptr = Some reply"
+  apply (clarsimp simp: obj_at'_def projectKO_eq opt_map_def)
+  done
+
 lemma obj_at_aligned':
-  fixes P :: "('a :: pspace_storable) \<Rightarrow> bool"
+  fixes P :: "'a :: pspace_storable \<Rightarrow> bool"
   assumes oat: "obj_at' P p s"
   and    oab: "\<And>(v :: 'a) (v' :: 'a). objBits v = objBits v'"
   shows "is_aligned p (objBits (obj :: 'a))"
   using oat
   apply (clarsimp simp add: obj_at'_def)
-  apply (clarsimp simp add: projectKO_def fail_def return_def
+  apply (clarsimp simp add: projectKO_def fail_def return_def oassert_opt_def
                             project_inject objBits_def[symmetric]
                      split: option.splits)
   apply (erule subst[OF oab])
@@ -2039,59 +2413,41 @@ lemma locateSlot_conv:
                          split: zombie_type.split cong: option.case_cong)
   done
 
+context
+begin
+
+private method typ_at_proof =
+  unfold obj_at'_real_def typ_at'_def ko_wp_at'_def,
+  (rule ext)+,
+  (rule iffI; clarsimp, case_tac ko; clarsimp simp: projectKO_opts_defs)
+
 lemma typ_at_tcb':
   "typ_at' TCBT = tcb_at'"
-  apply (rule ext)+
-  apply (simp add: obj_at'_real_def typ_at'_def)
-  apply (simp add: ko_wp_at'_def)
-  apply (rule iffI)
-   apply clarsimp
-   apply (case_tac ko)
-   apply (auto simp: projectKO_opt_tcb)[9]
-  apply (case_tac ko)
-  apply (auto simp: projectKO_opt_tcb)
-  done
+  by typ_at_proof
 
-lemma typ_at_ep:
+lemma typ_at_ep:  (* FIXME: rename to ' *)
   "typ_at' EndpointT = ep_at'"
-  apply (rule ext)+
-  apply (simp add: obj_at'_real_def typ_at'_def)
-  apply (simp add: ko_wp_at'_def)
-  apply (rule iffI)
-   apply clarsimp
-   apply (case_tac ko)
-   apply (auto simp: projectKO_opt_ep)[9]
-  apply (case_tac ko)
-  apply (auto simp: projectKO_opt_ep)
-  done
+  by typ_at_proof
 
-lemma typ_at_ntfn:
+lemma typ_at_ntfn: (* FIXME: rename to ' *)
   "typ_at' NotificationT = ntfn_at'"
-  apply (rule ext)+
-  apply (simp add: obj_at'_real_def typ_at'_def)
-  apply (simp add: ko_wp_at'_def)
-  apply (rule iffI)
-   apply clarsimp
-   apply (case_tac ko)
-   apply (auto simp: projectKO_opt_ntfn)[8]
-  apply clarsimp
-  apply (case_tac ko)
-  apply (auto simp: projectKO_opt_ntfn)
-  done
+  by typ_at_proof
 
-lemma typ_at_cte:
+lemma typ_at_cte: (* FIXME: rename to ' *)
   "typ_at' CTET = real_cte_at'"
-  apply (rule ext)+
-  apply (simp add: obj_at'_real_def typ_at'_def)
-  apply (simp add: ko_wp_at'_def)
-  apply (rule iffI)
-   apply clarsimp
-   apply (case_tac ko)
-   apply (auto simp: projectKO_opt_cte)[8]
-  apply clarsimp
-  apply (case_tac ko)
-  apply (auto simp: projectKO_opt_cte)
-  done
+  by typ_at_proof
+
+lemma typ_at_reply':
+  "typ_at' ReplyT = reply_at'"
+  by typ_at_proof
+
+lemma typ_at_sc':
+  "typ_at' SchedContextT = sc_at'"
+  by typ_at_proof
+
+lemmas typ_ats' = typ_at_sc' typ_at_reply' typ_at_cte typ_at_ntfn typ_at_ep typ_at_tcb'
+
+end
 
 lemma cte_at_typ':
   "cte_at' c = (\<lambda>s. typ_at' CTET c s \<or> (\<exists>n. typ_at' TCBT (c - n) s \<and> n \<in> dom tcb_cte_cases))"
@@ -2102,52 +2458,189 @@ proof -
   have Q: "\<And>P f. (\<exists>x. (\<exists>y. x = f y) \<and> P x) = (\<exists>y. P (f y))"
     by fastforce
   show ?thesis
-    by (fastforce simp: cte_wp_at_cases' obj_at'_real_def typ_at'_def
+    by (fastforce simp: cte_wp_at_cases' obj_at'_real_def typ_at'_def word_bits_def
                         ko_wp_at'_def objBits_simps' P Q conj_comms cte_level_bits_def)
 qed
 
-lemma typ_at_lift_tcb':
-  "\<lbrace>typ_at' TCBT p\<rbrace> f \<lbrace>\<lambda>_. typ_at' TCBT p\<rbrace> \<Longrightarrow> \<lbrace>tcb_at' p\<rbrace> f \<lbrace>\<lambda>_. tcb_at' p\<rbrace>"
+lemma typ_at_lift_tcb'_strong:
+  "f \<lbrace>\<lambda>s. P (typ_at' TCBT p s)\<rbrace> \<Longrightarrow> f \<lbrace>\<lambda>s. P (tcb_at' p s)\<rbrace>"
   by (simp add: typ_at_tcb')
 
-lemma typ_at_lift_ep':
-  "\<lbrace>typ_at' EndpointT p\<rbrace> f \<lbrace>\<lambda>_. typ_at' EndpointT p\<rbrace> \<Longrightarrow> \<lbrace>ep_at' p\<rbrace> f \<lbrace>\<lambda>_. ep_at' p\<rbrace>"
+lemma typ_at_lift_ep'_strong:
+  "f \<lbrace>\<lambda>s. P (typ_at' EndpointT p s)\<rbrace> \<Longrightarrow> f \<lbrace>\<lambda>s. P (ep_at' p s)\<rbrace>"
   by (simp add: typ_at_ep)
 
-lemma typ_at_lift_ntfn':
-  "\<lbrace>typ_at' NotificationT p\<rbrace> f \<lbrace>\<lambda>_. typ_at' NotificationT p\<rbrace> \<Longrightarrow> \<lbrace>ntfn_at' p\<rbrace> f \<lbrace>\<lambda>_. ntfn_at' p\<rbrace>"
+lemma typ_at_lift_ntfn'_strong:
+  "f \<lbrace>\<lambda>s. P (typ_at' NotificationT p s)\<rbrace> \<Longrightarrow> f \<lbrace>\<lambda>s. P (ntfn_at' p s)\<rbrace>"
   by (simp add: typ_at_ntfn)
 
-lemma typ_at_lift_cte':
-  "\<lbrace>typ_at' CTET p\<rbrace> f \<lbrace>\<lambda>_. typ_at' CTET p\<rbrace> \<Longrightarrow> \<lbrace>real_cte_at' p\<rbrace> f \<lbrace>\<lambda>_. real_cte_at' p\<rbrace>"
+lemma typ_at_lift_cte'_strong:
+  "f \<lbrace>\<lambda>s. P (typ_at' CTET p s)\<rbrace> \<Longrightarrow> f \<lbrace>\<lambda>s. P (real_cte_at' p s)\<rbrace>"
   by (simp add: typ_at_cte)
 
+lemma typ_at_lift_sc'_strong:
+  "f \<lbrace>\<lambda>s. P (typ_at' SchedContextT p s)\<rbrace> \<Longrightarrow> f \<lbrace>\<lambda>s. P (sc_at' p s)\<rbrace>"
+  by (simp add: typ_ats')
+
+lemma typ_at_lift_reply'_strong:
+  "f \<lbrace>\<lambda>s. P (typ_at' ReplyT p s)\<rbrace> \<Longrightarrow> f \<lbrace>\<lambda>s. P (reply_at' p s)\<rbrace>"
+  by (simp add: typ_ats')
+
 lemma typ_at_lift_cte_at':
-  assumes x: "\<And>T p. \<lbrace>typ_at' T p\<rbrace> f \<lbrace>\<lambda>rv. typ_at' T p\<rbrace>"
-  shows      "\<lbrace>cte_at' c\<rbrace> f \<lbrace>\<lambda>rv. cte_at' c\<rbrace>"
+  assumes x: "\<And>P T p. f \<lbrace>\<lambda>s. P (typ_at' T p s)\<rbrace>"
+  shows      "f \<lbrace>\<lambda>s. P (cte_at' c s)\<rbrace>"
   apply (simp only: cte_at_typ')
-  apply (wp hoare_vcg_disj_lift hoare_vcg_ex_lift x)
+  apply (rule P_bool_lift[where P=P])
+   apply (wpsimp wp: hoare_vcg_disj_lift hoare_vcg_ex_lift hoare_vcg_all_lift x)+
   done
 
-lemma typ_at_lift_page_table_at':
-  assumes x: "\<And>T p. f \<lbrace>typ_at' T p\<rbrace>"
-  shows "f \<lbrace>page_table_at' p\<rbrace>"
-  unfolding page_table_at'_def
-  by (wp hoare_vcg_all_lift x)
+lemma typ_at_lift_page_table_at'_strong:
+  "(\<And>p. f \<lbrace>\<lambda>s. P (typ_at' (ArchT PTET) p s)\<rbrace>) \<Longrightarrow> f \<lbrace>\<lambda>s. P (page_table_at' p s)\<rbrace>"
+  unfolding page_table_at'_def All_less_Ball
+  apply (rule P_bool_lift[where P=P])
+  apply (wpsimp wp: hoare_vcg_const_Ball_lift hoare_vcg_bex_lift hoare_vcg_imp_lift
+                    hoare_vcg_all_lift hoare_vcg_ex_lift
+         | fastforce)+
+  done
+
+lemma typ_at_lift_valid_tcb_state'_strong:
+  assumes ep: "\<And>p. f \<lbrace>\<lambda>s. P (typ_at' EndpointT p s)\<rbrace>"
+      and reply: "\<And>p. f \<lbrace>\<lambda>s. P (typ_at' ReplyT p s)\<rbrace>"
+      and ntfn: "\<And>p. f \<lbrace>\<lambda>s. P (typ_at' NotificationT p s)\<rbrace>"
+  shows "f \<lbrace>\<lambda>s. P (valid_tcb_state' st s)\<rbrace>"
+  unfolding valid_tcb_state'_def valid_bound_reply'_def
+  apply (case_tac st ; clarsimp split: option.splits,
+         wpsimp wp: hoare_vcg_imp_lift' hoare_vcg_all_lift hoare_vcg_conj_lift_N[where N=P]
+                    typ_at_lift_ep'_strong[OF ep] typ_at_lift_reply'_strong[OF reply]
+                    typ_at_lift_ntfn'_strong[OF ntfn])
+  done
+
+lemma typ_at_lift_frame_at'_strong:
+  assumes "\<And>P T p. f \<lbrace>\<lambda>s. P (typ_at' T p s)\<rbrace>"
+  shows "f \<lbrace>\<lambda>s. P (frame_at' p sz d s)\<rbrace>"
+  unfolding frame_at'_def
+  apply (rule P_bool_lift[where P=P])
+   apply (wpsimp wp: hoare_vcg_all_lift hoare_vcg_const_imp_lift assms hoare_vcg_ex_lift
+          split_del: if_split)+
+  done
+
+lemmas typ_at_lifts_strong =
+  typ_at_lift_tcb'_strong typ_at_lift_ep'_strong
+  typ_at_lift_ntfn'_strong typ_at_lift_cte'_strong
+  typ_at_lift_reply'_strong typ_at_lift_sc'_strong
+  typ_at_lift_valid_tcb_state'_strong
+  typ_at_lift_page_table_at'_strong
+  typ_at_lift_frame_at'_strong
 
 lemma ko_wp_typ_at':
   "ko_wp_at' P p s \<Longrightarrow> \<exists>T. typ_at' T p s"
   by (clarsimp simp: typ_at'_def ko_wp_at'_def)
 
 lemma koType_obj_range':
-  "koTypeOf k = koTypeOf k' \<Longrightarrow> obj_range' p k = obj_range' p k'"
+  "koTypeOf k = koTypeOf k' \<Longrightarrow> koTypeOf k = SchedContextT \<longrightarrow> objBitsKO k = objBitsKO k' \<Longrightarrow> obj_range' p k = obj_range' p k'"
   apply (rule ccontr)
   apply (simp add: obj_range'_def objBitsKO_def archObjSize_def
             split: kernel_object.splits arch_kernel_object.splits)
   done
 
+lemma typ_at_lift_valid_irq_node':
+  assumes P: "\<And>P T p. \<lbrace>\<lambda>s. P (typ_at' T p s)\<rbrace> f \<lbrace>\<lambda>rv s. P (typ_at' T p s)\<rbrace>"
+  shows      "\<lbrace>valid_irq_node' p\<rbrace> f \<lbrace>\<lambda>_. valid_irq_node' p\<rbrace>"
+  apply (simp add: valid_irq_node'_def)
+  apply (wp hoare_vcg_all_lift P typ_at_lifts_strong)
+  done
+
+lemma valid_dom_schedule'_lift:
+  assumes dsi: "\<And>Q. \<lbrace>\<lambda>s. Q (ksDomScheduleIdx s)\<rbrace> f \<lbrace>\<lambda>rv s. Q (ksDomScheduleIdx s)\<rbrace>"
+  assumes ds: "\<And>Q. \<lbrace>\<lambda>s. Q (ksDomSchedule s)\<rbrace> f \<lbrace>\<lambda>rv s. Q (ksDomSchedule s)\<rbrace>"
+    shows "\<lbrace>\<lambda>s. valid_dom_schedule' s\<rbrace> f \<lbrace>\<lambda>rv. valid_dom_schedule'\<rbrace>"
+   unfolding valid_dom_schedule'_def
+   by (wpsimp wp: dsi ds)
+
+lemma valid_bound_tcb_lift:
+  "(\<And>T p. f \<lbrace>typ_at' T p\<rbrace>) \<Longrightarrow> f \<lbrace>valid_bound_tcb' tcb\<rbrace>"
+  by (auto simp: valid_bound_tcb'_def valid_def typ_ats'[symmetric] split: option.splits)
+
+lemma valid_bound_sc_lift:
+  "(\<And>T p. f \<lbrace>typ_at' T p\<rbrace>) \<Longrightarrow> f \<lbrace>valid_bound_sc' tcb\<rbrace>"
+  by (auto simp: valid_bound_obj'_def valid_def typ_ats'[symmetric] split: option.splits)
+
+lemma valid_bound_reply_lift:
+  "(\<And>T p. f \<lbrace>typ_at' T p\<rbrace>) \<Longrightarrow> f \<lbrace>valid_bound_reply' tcb\<rbrace>"
+  by (auto simp: valid_bound_tcb'_def valid_def typ_ats'[symmetric] split: option.splits)
+
+lemma valid_bound_ntfn_lift:
+  "(\<And>T p. f \<lbrace>typ_at' T p\<rbrace>) \<Longrightarrow> f \<lbrace>valid_bound_ntfn' ntfn\<rbrace>"
+  by (auto simp: valid_bound_obj'_def valid_def typ_ats'[symmetric] split: option.splits)
+
+lemma valid_ntfn_lift':
+  "(\<And>T p. f \<lbrace>typ_at' T p\<rbrace>) \<Longrightarrow> f \<lbrace>valid_ntfn' ntfn\<rbrace>"
+  unfolding valid_ntfn'_def
+  apply (cases "ntfnObj ntfn"; clarsimp)
+    apply (wpsimp wp: valid_bound_tcb_lift valid_bound_sc_lift)
+   apply (wpsimp wp: valid_bound_tcb_lift valid_bound_sc_lift)
+  apply (wpsimp wp: hoare_vcg_ball_lift typ_at_lift_tcb'_strong[where P=id, simplified])
+   apply (wpsimp wp: valid_bound_tcb_lift valid_bound_sc_lift)
+  apply simp
+  done
+
+lemma valid_sc_lift':
+  "(\<And>T p. f \<lbrace>typ_at' T p\<rbrace>) \<Longrightarrow> f \<lbrace>valid_sched_context' sc\<rbrace>"
+  unfolding valid_sched_context'_def
+  by (wpsimp wp: valid_bound_ntfn_lift valid_bound_tcb_lift valid_bound_reply_lift)
+
+context begin
+\<comment>\<open> We're using @{command ML_goal} here because there are two useful formulations
+    of typ_at lifting lemmas and we do not want to write all of the possibilities
+    out by hand. If we use typ_at_lift_tcb' as an example, then the first is
+    @{term "\<lbrace>\<lambda>s. P (typ_at' TCBT p s)\<rbrace> f \<lbrace>\<lambda>_ s. P (typ_at' TCBT p s)\<rbrace>
+            \<Longrightarrow> \<lbrace>\<lambda>s. P (tcb_at' p s)\<rbrace> f \<lbrace>\<lambda>_ s. P (tcb_at' p s)\<rbrace>"} and the second is
+    @{term "(\<And>P. \<lbrace>\<lambda>s. P (typ_at' TCBT p s)\<rbrace> f \<lbrace>\<lambda>_ s. P (typ_at' TCBT p s)\<rbrace>)
+            \<Longrightarrow> \<lbrace>\<lambda>s. P (tcb_at' p s)\<rbrace> f \<lbrace>\<lambda>_ s. P (tcb_at' p s)\<rbrace>"}.
+    The first form is stronger, and therefore preferred for backward reasoning
+    using rule. However, since the P in the premise is free in the first form,
+    forward unification using the OF attribute produces flex-flex pairs which
+    causes problems. The second form avoids the unification issue by demanding
+    that there is a P that is free in the lemma supplied to the OF attribute.
+    However, it can only be applied if @{term f} preserves both
+    @{term "typ_at' TCBT p s"} and @{term "\<not> typ_at' TCBT p s"}.
+    The following @{command ML_goal} generates lemmas of the second form based on
+    the previously proven stronger lemmas of the first form. \<close>
+ML \<open>
+local
+  val strong_thms = @{thms typ_at_lifts_strong[no_vars]};
+  fun abstract_P term = Logic.all (Free ("P", @{typ "bool \<Rightarrow> bool"})) term
+  fun abstract thm =
+    let
+      val prems = List.map abstract_P (Thm.prems_of thm);
+      fun imp [] = Thm.concl_of thm
+        | imp (p :: pms) = @{const Pure.imp} $ p $ imp pms
+    in
+      imp prems
+    end
+in
+  val typ_at_lifts_internal_goals = List.map abstract strong_thms
+end
+\<close>
+
+private ML_goal typ_at_lifts_internal:
+  \<open>typ_at_lifts_internal_goals\<close>
+  by (auto simp: typ_at_lifts_strong)
+
+lemmas typ_at_lifts = typ_at_lifts_internal
+                      typ_at_lift_cte_at'
+                      valid_bound_tcb_lift
+                      valid_bound_reply_lift
+                      valid_bound_sc_lift
+                      valid_bound_ntfn_lift
+                      valid_ntfn_lift'
+                      valid_sc_lift'
+                      typ_at_lift_frame_at'_strong
+end
+
 lemma typ_at_lift_valid_untyped':
   assumes P: "\<And>T p. \<lbrace>\<lambda>s. \<not>typ_at' T p s\<rbrace> f \<lbrace>\<lambda>rv s. \<not>typ_at' T p s\<rbrace>"
+  assumes sz: "\<And>p n. \<lbrace>\<lambda>s. sc_at'_n n p s\<rbrace> f \<lbrace>\<lambda>rv s. sc_at'_n n p s\<rbrace>"
   shows "\<lbrace>\<lambda>s. valid_untyped' d p n idx s\<rbrace> f \<lbrace>\<lambda>rv s. valid_untyped' d p n idx s\<rbrace>"
   apply (clarsimp simp: valid_untyped'_def split del:if_split)
   apply (rule hoare_vcg_all_lift)
@@ -2164,68 +2657,111 @@ lemma typ_at_lift_valid_untyped':
   apply (clarsimp simp: typ_at'_def ko_wp_at'_def simp del:atLeastAtMost_iff)
   apply (elim disjE)
     apply (clarsimp simp:psubset_eq simp del:atLeastAtMost_iff)
-    apply (drule_tac p=ptr' in koType_obj_range')
-    apply (erule impE)
-    apply simp
+   apply (frule_tac p=ptr' in koType_obj_range', clarsimp)
+    apply (fastforce simp: ko_wp_at'_def dest!: use_valid [OF _ sz])
    apply simp
-  apply (drule_tac p = ptr' in koType_obj_range')
-  apply (clarsimp split:if_splits)
+  apply (frule_tac p = ptr' in koType_obj_range', clarsimp)
+   apply (fastforce simp: ko_wp_at'_def dest!: use_valid [OF _ sz])
+  apply simp
   done
-
-lemma typ_at_lift_asid_at':
-  "(\<And>T p. \<lbrace>typ_at' T p\<rbrace> f \<lbrace>\<lambda>_. typ_at' T p\<rbrace>) \<Longrightarrow> \<lbrace>asid_pool_at' p\<rbrace> f \<lbrace>\<lambda>_. asid_pool_at' p\<rbrace>"
-  by assumption
-
-lemma typ_at_lift_frame_at':
-  assumes "\<And>T p. f \<lbrace>typ_at' T p\<rbrace>"
-  shows "f \<lbrace>frame_at' p sz d\<rbrace>"
-  unfolding frame_at'_def
-  by (wpsimp wp: hoare_vcg_all_lift hoare_vcg_const_imp_lift assms split_del: if_split)
 
 lemma typ_at_lift_valid_cap':
   assumes P: "\<And>P T p. \<lbrace>\<lambda>s. P (typ_at' T p s)\<rbrace> f \<lbrace>\<lambda>rv s. P (typ_at' T p s)\<rbrace>"
+  assumes sz: "\<And>p n. \<lbrace>\<lambda>s. sc_at'_n n p s\<rbrace> f \<lbrace>\<lambda>rv s. sc_at'_n n p s\<rbrace>"
   shows      "\<lbrace>\<lambda>s. valid_cap' cap s\<rbrace> f \<lbrace>\<lambda>rv s. valid_cap' cap s\<rbrace>"
   including no_pre
   apply (simp add: valid_cap'_def)
   apply wp
   apply (case_tac cap;
-         simp add: valid_cap'_def P[of id, simplified] typ_at_lift_tcb'
-                   hoare_vcg_prop typ_at_lift_ep'
-                   typ_at_lift_ntfn' typ_at_lift_cte_at'
-                   hoare_vcg_conj_lift [OF typ_at_lift_cte_at'])
+         wpsimp wp: valid_cap'_def P typ_at_lifts_strong
+                    hoare_vcg_prop  typ_at_lift_cte_at'
+                    hoare_vcg_conj_lift [OF typ_at_lift_cte_at']
+                    hoare_vcg_conj_lift)
      apply (rename_tac zombie_type nat)
      apply (case_tac zombie_type; simp)
-      apply (wp typ_at_lift_tcb' P hoare_vcg_all_lift typ_at_lift_cte')+
+      apply (wp typ_at_lifts_strong[where P=id, simplified] P
+                hoare_vcg_all_lift)+
     apply (rename_tac arch_capability)
     apply (case_tac arch_capability,
-           simp_all add: P[of id, simplified] vspace_table_at'_defs
+           simp_all add: P [where P=id, simplified] page_table_at'_def
                          hoare_vcg_prop All_less_Ball
-                    split del: if_split)
-       apply (wp hoare_vcg_const_Ball_lift P typ_at_lift_valid_untyped'
-                 hoare_vcg_all_lift typ_at_lift_cte' typ_at_lift_frame_at')+
+              split del: if_split)
+       apply (wp hoare_vcg_const_Ball_lift P typ_at_lift_valid_untyped' sz
+                 hoare_vcg_all_lift typ_at_lifts_strong)+
   done
 
-
-lemma typ_at_lift_valid_irq_node':
+lemma typ_at'_valid_obj'_lift:
   assumes P: "\<And>P T p. \<lbrace>\<lambda>s. P (typ_at' T p s)\<rbrace> f \<lbrace>\<lambda>rv s. P (typ_at' T p s)\<rbrace>"
-  shows      "\<lbrace>valid_irq_node' p\<rbrace> f \<lbrace>\<lambda>_. valid_irq_node' p\<rbrace>"
-  apply (simp add: valid_irq_node'_def)
-  apply (wp hoare_vcg_all_lift P typ_at_lift_cte')
+  assumes sz: "\<And>n p. \<lbrace>\<lambda>s. sc_at'_n n p s\<rbrace> f \<lbrace>\<lambda>rv s. sc_at'_n n p s\<rbrace>"
+  notes [wp] = hoare_vcg_all_lift hoare_vcg_imp_lift' hoare_vcg_const_Ball_lift
+               typ_at_lifts[OF P] typ_at_lift_valid_cap'[OF P]
+  shows      "\<lbrace>\<lambda>s. valid_obj' obj s\<rbrace> f \<lbrace>\<lambda>rv s. valid_obj' obj s\<rbrace>"
+  apply (cases obj; simp add: valid_obj'_def hoare_TrueI)
+       apply (rename_tac endpoint)
+       apply (case_tac endpoint; simp add: valid_ep'_def, wp)
+      apply (rename_tac notification)
+      apply (case_tac "ntfnObj notification";
+              simp add: valid_ntfn'_def split: option.splits;
+              (wpsimp|rule conjI)+)
+     apply (rename_tac tcb)
+     apply (case_tac "tcbState tcb";
+            simp add: valid_tcb'_def valid_tcb_state'_def split_def;
+            wpsimp wp: sz)
+    apply (wpsimp simp: valid_cte'_def sz)
+   apply (rename_tac arch_kernel_object)
+   apply (case_tac arch_kernel_object; wpsimp wp: sz)
+  apply (wpsimp simp: valid_reply'_def)
   done
 
-lemma valid_bound_tcb_lift:
-  "(\<And>T p. \<lbrace>typ_at' T p\<rbrace> f \<lbrace>\<lambda>_. typ_at' T p\<rbrace>) \<Longrightarrow>
-  \<lbrace>valid_bound_tcb' tcb\<rbrace> f \<lbrace>\<lambda>_. valid_bound_tcb' tcb\<rbrace>"
-  by (auto simp: valid_bound_tcb'_def valid_def typ_at_tcb'[symmetric] split: option.splits)
+lemma typ_at'_valid_sched_context'_lift:
+  assumes P: "\<And>P T p. \<lbrace>\<lambda>s. P (typ_at' T p s)\<rbrace> f \<lbrace>\<lambda>rv s. P (typ_at' T p s)\<rbrace>"
+  assumes sz: "\<And>n p. \<lbrace>\<lambda>s. sc_at'_n n p s\<rbrace> f \<lbrace>\<lambda>rv s. sc_at'_n n p s\<rbrace>"
+  notes [wp] = hoare_vcg_all_lift hoare_vcg_imp_lift' hoare_vcg_const_Ball_lift
+               typ_at_lifts[OF P] typ_at_lift_valid_cap'[OF P]
+  shows      "\<lbrace>\<lambda>s. valid_sched_context' ko s\<rbrace> f \<lbrace>\<lambda>rv s. valid_sched_context' ko s\<rbrace>"
+  by (wpsimp simp: valid_sched_context'_def)
 
-lemmas typ_at_lifts = typ_at_lift_tcb' typ_at_lift_ep'
-                      typ_at_lift_ntfn' typ_at_lift_cte'
-                      typ_at_lift_cte_at'
-                      typ_at_lift_page_table_at'
-                      typ_at_lift_asid_at'
-                      typ_at_lift_valid_untyped'
-                      typ_at_lift_valid_cap'
-                      valid_bound_tcb_lift
+lemmas typ_at_sc_at'_n_lifts =
+  typ_at_lift_valid_untyped' typ_at_lift_valid_cap' typ_at'_valid_obj'_lift
+  typ_at'_valid_obj'_lift[where obj="KOEndpoint ko" for ko, simplified valid_obj'_def kernel_object.case]
+  typ_at'_valid_obj'_lift[where obj="KONotification ko" for ko, simplified valid_obj'_def kernel_object.case]
+  typ_at'_valid_obj'_lift[where obj="KOTCB ko" for ko, simplified valid_obj'_def kernel_object.case]
+  typ_at'_valid_obj'_lift[where obj="KOCTE ko" for ko, simplified valid_obj'_def kernel_object.case]
+  typ_at'_valid_obj'_lift[where obj="KOArch ko" for ko, simplified valid_obj'_def kernel_object.case]
+  typ_at'_valid_obj'_lift[where obj="KOReply ko" for ko, simplified valid_obj'_def kernel_object.case]
+  typ_at'_valid_sched_context'_lift
+
+lemmas typ_at_lifts_all = typ_at_lifts typ_at_sc_at'_n_lifts
+
+end
+
+locale typ_at_props' =
+  fixes f :: "'a kernel"
+  assumes typ': "f \<lbrace>\<lambda>s. P (typ_at' T p' s)\<rbrace>"
+begin
+
+lemmas typ_at_lifts'[wp] = typ_at_lifts[REPEAT [OF typ']]
+
+end
+
+locale typ_at_all_props' = typ_at_props' +
+  assumes scs: "f \<lbrace>\<lambda>s. Q (sc_at'_n n p s)\<rbrace>"
+begin
+
+lemmas typ_at_sc_at'_n_lifts'[wp] = typ_at_sc_at'_n_lifts[OF typ' scs]
+
+context begin
+(* We want to enforce that typ_at_sc_at'_n_lifts' only contains lemmas that have no
+   assumptions. The following thm statements should fail if this is not true. *)
+private lemmas check_valid_internal = iffD1[OF refl, where P="valid p g q" for p g q]
+thm typ_at_lifts'[atomized, THEN check_valid_internal]
+thm typ_at_sc_at'_n_lifts'[atomized, THEN check_valid_internal]
+end
+
+end
+
+(* we expect typ_at' and sc_at'_n lemmas to be [wp], so this should be easy: *)
+method typ_at_props' = unfold_locales; wp?
 
 lemma mdb_next_unfold:
   "s \<turnstile> c \<leadsto> c' = (\<exists>z. s c = Some z \<and> c' = mdbNext (cteMDBNode z))"
@@ -2378,8 +2914,7 @@ lemma valid_mdb_ctesE [elim]:
     \<lbrakk> valid_dlist m; no_0 m; mdb_chain_0 m; valid_badges m;
       caps_contained' m; mdb_chunked m; untyped_mdb' m;
       untyped_inc' m; valid_nullcaps m; ut_revocable' m;
-      class_links m; distinct_zombies m; irq_control m;
-      reply_masters_rvk_fb m \<rbrakk>
+      class_links m; distinct_zombies m; irq_control m \<rbrakk>
           \<Longrightarrow> P\<rbrakk> \<Longrightarrow> P"
   unfolding valid_mdb_ctes_def by auto
 
@@ -2387,12 +2922,10 @@ lemma valid_mdb_ctesI [intro]:
   "\<lbrakk>valid_dlist m; no_0 m; mdb_chain_0 m; valid_badges m;
     caps_contained' m; mdb_chunked m; untyped_mdb' m;
     untyped_inc' m; valid_nullcaps m; ut_revocable' m;
-    class_links m; distinct_zombies m; irq_control m;
-    reply_masters_rvk_fb m \<rbrakk>
+    class_links m; distinct_zombies m; irq_control m \<rbrakk>
   \<Longrightarrow> valid_mdb_ctes m"
   unfolding valid_mdb_ctes_def by auto
 
-end
 locale PSpace_update_eq =
   fixes f :: "kernel_state \<Rightarrow> kernel_state"
   assumes pspace: "ksPSpace (f s) = ksPSpace s"
@@ -2432,6 +2965,18 @@ lemma valid_objs_update [iff]:
   apply (fastforce intro: valid_obj'_pspaceI simp: pspace)
   done
 
+lemma valid_objs_size_update [iff]:
+  "valid_objs_size' (f s) = valid_objs_size' s"
+  apply (simp add: valid_objs_size'_def pspace)
+  apply (fastforce intro: valid_obj_size'_pspaceI simp: pspace)
+  done
+
+lemma valid_replies'_update [iff]:
+  "valid_replies' (f s) = valid_replies' s"
+  apply (simp add: valid_replies'_def pspace)
+  apply (auto simp: pspace pred_tcb_at'_def)
+  done
+
 lemma pspace_aligned_update [iff]:
   "pspace_aligned' (f s) = pspace_aligned' s"
   by (simp add: pspace pspace_aligned'_def)
@@ -2447,6 +2992,14 @@ lemma pspace_in_kernel_mappings_update [iff]:
 lemma pspace_distinct_update [iff]:
   "pspace_distinct' (f s) = pspace_distinct' s"
   by (simp add: pspace pspace_distinct'_def ps_clear_def)
+
+lemma pspace_bounded_update [iff]:
+  "pspace_bounded' (f s) = pspace_bounded' s"
+  by (simp add: pspace pspace_bounded'_def)
+
+lemma pspace_no_overlap'_update [iff]:
+  "pspace_no_overlap' p sz (f s) = pspace_no_overlap' p sz s"
+  by (simp add: pspace pspace_no_overlap'_def ps_clear_def)
 
 lemma pred_tcb_at_update [iff]:
   "pred_tcb_at' proj P p (f s) = pred_tcb_at' proj P p s"
@@ -2587,6 +3140,26 @@ interpretation ready_queue_bitmap2_update:
   P_Arch_Idle_Int_Cur_update_eq "ksReadyQueuesL2Bitmap_update f"
   by unfold_locales auto
 
+interpretation reprogramTime_update:
+  P_Arch_Idle_Int_Cur_update_eq "ksReprogramTimer_update f"
+  by unfold_locales auto
+
+interpretation ksReleaseQueue_update:
+  P_Arch_Idle_Int_Cur_update_eq "ksReleaseQueue_update f"
+  by unfold_locales auto
+
+interpretation ksConsumedTime_update:
+  P_Arch_Idle_Int_Cur_update_eq "ksConsumedTime_update f"
+  by unfold_locales auto
+
+interpretation ksCurTime_update:
+  P_Arch_Idle_Int_Cur_update_eq "ksCurTime_update f"
+  by unfold_locales auto
+
+interpretation ksCurSc_update:
+  P_Arch_Idle_Int_Cur_update_eq "ksCurSc_update f"
+  by unfold_locales auto
+
 interpretation cur_thread_update':
   P_Arch_Idle_Int_update_eq "ksCurThread_update f"
   by unfold_locales auto
@@ -2644,6 +3217,11 @@ lemma ko_wp_at_norm:
   "ko_wp_at' P p s \<Longrightarrow> \<exists>ko. P ko \<and> ko_wp_at' ((=) ko) p s"
   by (auto simp add: ko_wp_at'_def)
 
+lemma ko_at_ko_wp_atD':
+  "\<lbrakk>ko_at' ko p s; ko_wp_at' P p s\<rbrakk> \<Longrightarrow> P (injectKO ko)"
+  apply (clarsimp simp: obj_at'_def ko_wp_at'_def projectKO_eq project_inject)
+  done
+
 lemma valid_mdb_machine_state [iff]:
   "valid_mdb' (ksMachineState_update f s) = valid_mdb' s"
   by (simp add: valid_mdb'_def)
@@ -2655,6 +3233,10 @@ lemma cte_wp_at_norm':
 lemma pred_tcb_at' [elim!]:
   "pred_tcb_at' proj P t s \<Longrightarrow> tcb_at' t s"
   by (auto simp add: pred_tcb_at'_def obj_at'_def)
+
+lemma pred_tcb_at'_True[simp]:
+  "pred_tcb_at' proj \<top> p s = tcb_at' p s"
+  by (clarsimp simp: pred_tcb_at'_def obj_at'_def)
 
 lemma valid_pspace_mdb' [elim!]:
   "valid_pspace' s \<Longrightarrow> valid_mdb' s"
@@ -2675,19 +3257,6 @@ lemma ex_cte_cap_to'_pres:
   done
 
 section "Relationship of Executable Spec to Kernel Configuration"
-
-text \<open>
-  Some values are set per kernel configuration (e.g. number of domains), but other related
-  values (e.g. maximum domain) are derived from storage constraints (e.g. bytes used).
-  To relate the two, we must look at the values of kernel configuration constants.
-  To allow the proofs to work for all permitted values of these constants, their definitions
-  should only be unfolded in this section, and the derived properties kept to a minimum.\<close>
-
-lemma le_maxDomain_eq_less_numDomains:
-  shows "x \<le> unat maxDomain \<longleftrightarrow> x < Kernel_Config.numDomains"
-        "y \<le> maxDomain \<longleftrightarrow> unat y < Kernel_Config.numDomains"
-  by (auto simp: Kernel_Config.numDomains_def maxDomain_def word_le_nat_alt)
-
 
 context begin interpretation Arch . (*FIXME: arch_split*)
 
@@ -2771,6 +3340,14 @@ lemma valid_queues_arch [simp]:
   "valid_queues (ksArchState_update f s) = valid_queues s"
   by (simp add: valid_queues_def valid_queues_no_bitmap_def bitmapQ_defs)
 
+lemma valid_release_queue_arch [simp]:
+  "valid_release_queue (ksArchState_update f s) = valid_release_queue s"
+  by (simp add: valid_release_queue_def)
+
+lemma valid_release_queue'_arch [simp]:
+  "valid_release_queue' (ksArchState_update f s) = valid_release_queue' s"
+  by (simp add: valid_release_queue'_def)
+
 lemma if_unsafe_then_cap_arch' [simp]:
   "if_unsafe_then_cap' (ksArchState_update f s) = if_unsafe_then_cap' s"
   by (simp add: if_unsafe_then_cap'_def ex_cte_cap_to'_def)
@@ -2790,6 +3367,14 @@ lemma sch_act_wf_machine_state [simp]:
 lemma valid_queues_machine_state [simp]:
   "valid_queues (ksMachineState_update f s) = valid_queues s"
   by (simp add: valid_queues_def valid_queues_no_bitmap_def bitmapQ_defs)
+
+lemma valid_release_queue_machine_state [simp]:
+  "valid_release_queue (ksMachineState_update f s) = valid_release_queue s"
+  by (simp add: valid_release_queue_def)
+
+lemma valid_release_queue'_machine_state [simp]:
+  "valid_release_queue' (ksMachineState_update f s) = valid_release_queue' s"
+  by (simp add: valid_release_queue'_def)
 
 lemma valid_queues_arch' [simp]:
   "valid_queues' (ksArchState_update f s) = valid_queues' s"
@@ -2832,6 +3417,14 @@ lemma valid_pspace_valid_objs'[elim!]:
   "valid_pspace' s \<Longrightarrow> valid_objs' s"
   by (simp add: valid_pspace'_def)
 
+lemma valid_pspace_valid_replies'[elim!]:
+  "valid_pspace' s \<Longrightarrow> valid_replies' s"
+  by (simp add: valid_pspace'_def)
+
+lemma valid_pspace_valid_objs_size'[elim!]:
+  "valid_pspace' s \<Longrightarrow> valid_objs_size' s"
+  by (simp add: valid_pspace'_def valid_objs'_valid_objs_size')
+
 declare badgeBits_def [simp]
 
 lemma simple_sane_strg:
@@ -2864,6 +3457,7 @@ lemma objBitsT_simps:
   "objBitsT NotificationT = ntfnSizeBits"
   "objBitsT CTET = cteSizeBits"
   "objBitsT TCBT = tcbBlockSizeBits"
+  "objBitsT ReplyT = replySizeBits"
   "objBitsT UserDataT = pageBits"
   "objBitsT UserDataDeviceT = pageBits"
   "objBitsT KernelDataT = pageBits"
@@ -2872,30 +3466,10 @@ lemma objBitsT_simps:
   unfolding objBitsT_def makeObjectT_def
   by (simp add: makeObject_simps objBits_simps bit_simps')+
 
-
-lemma objBitsT_koTypeOf :
-  "(objBitsT (koTypeOf ko)) = objBitsKO ko"
-  apply (cases ko; simp add: objBits_simps objBitsT_simps)
-  apply (rename_tac arch_kernel_object)
-  apply (case_tac arch_kernel_object; simp add: archObjSize_def objBitsT_simps bit_simps')
-  done
-
-lemma typ_at_aligned':
-  "\<lbrakk> typ_at' tp p s \<rbrakk> \<Longrightarrow> is_aligned p (objBitsT tp)"
-  by (clarsimp simp add: typ_at'_def ko_wp_at'_def objBitsT_koTypeOf)
-
 lemma valid_queues_obj_at'D:
    "\<lbrakk> t \<in> set (ksReadyQueues s (d, p)); valid_queues s \<rbrakk>
         \<Longrightarrow> obj_at' (inQ d p) t s"
-  apply (unfold valid_queues_def valid_queues_no_bitmap_def)
-  apply (elim conjE)
-  apply (drule_tac x=d in spec)
-  apply (drule_tac x=p in spec)
-  apply (clarsimp)
-  apply (drule(1) bspec)
-  apply (erule obj_at'_weakenE)
-  apply (clarsimp)
-  done
+  by (fastforce simp: valid_queues_def valid_queues_no_bitmap_def)
 
 lemma obj_at'_and:
   "obj_at' (P and P') t s = (obj_at' P t s \<and> obj_at' P' t s)"
@@ -2938,20 +3512,28 @@ lemma obj_at'_ko_at'_prop:
   "ko_at' ko t s \<Longrightarrow> obj_at' P t s = P ko"
   by (drule obj_at_ko_at', clarsimp simp: obj_at'_def)
 
+lemma obj_at'_imp:
+  fixes P Q :: "'a :: pspace_storable \<Rightarrow> bool"
+  shows
+  "(obj_at' (\<lambda>rv. P rv \<longrightarrow> Q rv) p s) =
+    (obj_at' (\<lambda>_ :: 'a. True) p s \<and> (obj_at' P p s \<longrightarrow> obj_at' Q p s))"
+  apply (rule iffI; clarsimp simp: obj_at'_def)
+  done
+
+lemma pred_tcb_at'_imp:
+  "pred_tcb_at' field (\<lambda>rv. P rv \<longrightarrow> Q rv) p s =
+    (tcb_at' p s \<and> (pred_tcb_at' field P p s \<longrightarrow> pred_tcb_at' field Q p s))"
+  apply (rule iffI; clarsimp simp: obj_at'_def pred_tcb_at'_def)
+  done
+
 lemma valid_queues_no_bitmap_def':
   "valid_queues_no_bitmap =
-     (\<lambda>s. \<forall>d p. (\<forall>t\<in>set (ksReadyQueues s (d, p)).
-                  obj_at' (inQ d p) t s \<and> st_tcb_at' runnable' t s) \<and>
-                  distinct (ksReadyQueues s (d, p)) \<and> (d > maxDomain \<or> p > maxPriority \<longrightarrow> ksReadyQueues s (d,p) = []))"
+     (\<lambda>s. \<forall>d p. (\<forall>t\<in>set (ksReadyQueues s (d, p)). obj_at' (inQ d p) t s) \<and>
+                (d > maxDomain \<or> p > maxPriority \<longrightarrow> ksReadyQueues s (d,p) = []))"
   apply (rule ext, rule iffI)
   apply (clarsimp simp: valid_queues_def valid_queues_no_bitmap_def obj_at'_and pred_tcb_at'_def o_def
                   elim!: obj_at'_weakenE)+
   done
-
-lemma valid_queues_running:
-  assumes Q: "t \<in> set(ksReadyQueues s (d, p))" "valid_queues s"
-  shows "st_tcb_at' runnable' t s"
-  using assms by (clarsimp simp add: valid_queues_def valid_queues_no_bitmap_def')
 
 lemma valid_refs'_cteCaps:
   "valid_refs' S (ctes_of s) = (\<forall>c \<in> ran (cteCaps_of s). S \<inter> capRange c = {})"
@@ -2971,41 +3553,41 @@ lemma cte_at_valid_cap_sizes_0:
   apply simp
   done
 
-lemma invs_valid_stateI' [elim!]:
-  "invs' s \<Longrightarrow> valid_state' s"
-  by (simp add: invs'_def)
-
-lemma tcb_at_invs' [elim!]:
-  "invs' s \<Longrightarrow> tcb_at' (ksCurThread s) s"
-  by (simp add: invs'_def cur_tcb'_def)
-
 lemma invs_valid_objs' [elim!]:
   "invs' s \<Longrightarrow> valid_objs' s"
-  by (simp add: invs'_def valid_state'_def valid_pspace'_def)
+  by (simp add: invs'_def valid_pspace'_def)
+
+lemma invs_valid_objs_size' [elim!]:
+  "invs' s \<Longrightarrow> valid_objs_size' s"
+  by (fastforce simp: invs'_def)
 
 lemma invs_pspace_aligned' [elim!]:
   "invs' s \<Longrightarrow> pspace_aligned' s"
-  by (simp add: invs'_def valid_state'_def valid_pspace'_def)
+  by (simp add: invs'_def valid_pspace'_def)
 
 lemma invs_pspace_distinct' [elim!]:
   "invs' s \<Longrightarrow> pspace_distinct' s"
-  by (simp add: invs'_def valid_state'_def valid_pspace'_def)
+  by (simp add: invs'_def valid_pspace'_def)
+
+lemma invs_pspace_bounded' [elim!]:
+  "invs' s \<Longrightarrow> pspace_bounded' s"
+  by (simp add: invs'_def valid_pspace'_def)
 
 lemma invs_valid_pspace' [elim!]:
   "invs' s \<Longrightarrow> valid_pspace' s"
-  by (simp add: invs'_def valid_state'_def)
+  by (simp add: invs'_def)
 
 lemma invs_arch_state' [elim!]:
   "invs' s \<Longrightarrow> valid_arch_state' s"
-  by (simp add: invs'_def valid_state'_def)
-
-lemma invs_cur' [elim!]:
-  "invs' s \<Longrightarrow> cur_tcb' s"
   by (simp add: invs'_def)
 
 lemma invs_mdb' [elim!]:
   "invs' s \<Longrightarrow> valid_mdb' s"
-  by (simp add: invs'_def valid_state'_def valid_pspace'_def)
+  by (simp add: invs'_def valid_pspace'_def)
+
+lemma invs_valid_replies'[elim!]:
+  "invs' s \<Longrightarrow> valid_replies' s"
+  by (simp add: invs'_def valid_pspace'_def)
 
 lemma valid_mdb_no_loops [elim!]:
   "valid_mdb_ctes m \<Longrightarrow> no_loops m"
@@ -3014,49 +3596,46 @@ lemma valid_mdb_no_loops [elim!]:
 lemma invs_no_loops [elim!]:
   "invs' s \<Longrightarrow> no_loops (ctes_of s)"
   apply (rule valid_mdb_no_loops)
-  apply (simp add: invs'_def valid_state'_def valid_pspace'_def valid_mdb'_def)
+  apply (simp add: invs'_def valid_pspace'_def valid_mdb'_def)
   done
 
 lemma invs_iflive'[elim!]:
   "invs' s \<Longrightarrow> if_live_then_nonz_cap' s"
-  by (simp add: invs'_def valid_state'_def)
+  by (simp add: invs'_def)
 
 lemma invs_unsafe_then_cap' [elim!]:
   "invs' s \<Longrightarrow> if_unsafe_then_cap' s"
-  by (simp add: invs'_def valid_state'_def)
-
-lemma invs_sym' [elim!]:
-  "invs' s \<Longrightarrow> sym_refs (state_refs_of' s)"
-  by (simp add: invs'_def valid_state'_def)
-
-lemma invs_sch_act_wf' [elim!]:
-  "invs' s \<Longrightarrow> sch_act_wf (ksSchedulerAction s) s"
-  by (simp add: invs'_def valid_state'_def)
+  by (simp add: invs'_def)
 
 lemma invs_queues [elim!]:
   "invs' s \<Longrightarrow> valid_queues s"
-  by (simp add: invs'_def valid_state'_def)
+  by (simp add: invs'_def)
 
-lemma invs_valid_idle'[elim!]:
-  "invs' s \<Longrightarrow> valid_idle' s"
-  by (fastforce simp: invs'_def valid_state'_def)
+lemma invs_queues'[elim!]:
+  "invs' s \<Longrightarrow> valid_queues' s"
+  by (simp add: invs'_def)
+
+lemma invs_valid_release_queue [elim!]:
+  "invs' s \<Longrightarrow> valid_release_queue s"
+  by (simp add: invs'_def)
+
+lemma invs_valid_release_queue' [elim!]:
+  "invs' s \<Longrightarrow> valid_release_queue' s"
+  by (simp add: invs'_def)
+
+lemma invs_sym_list_refs_of_replies'[elim!]:
+  "invs' s \<Longrightarrow> sym_refs (list_refs_of_replies' s)"
+  by (simp add: invs'_def)
 
 lemma invs_valid_global'[elim!]:
   "invs' s \<Longrightarrow> valid_global_refs' s"
-  by (fastforce simp: invs'_def valid_state'_def)
-
-lemma invs'_invs_no_cicd:
-  "invs' s \<Longrightarrow> all_invs_but_ct_idle_or_in_cur_domain' s"
-  by (simp add: invs'_to_invs_no_cicd'_def)
+  by (fastforce simp: invs'_def)
 
 lemma invs_valid_queues'_strg:
   "invs' s \<longrightarrow> valid_queues' s"
-  by (clarsimp simp: invs'_def valid_state'_def)
+  by (clarsimp simp: invs'_def)
 
 lemmas invs_valid_queues'[elim!] = invs_valid_queues'_strg[rule_format]
-
-lemma einvs_valid_etcbs: "einvs s \<longrightarrow> valid_etcbs s"
-  by (clarsimp simp: valid_sched_def)
 
 lemma invs'_bitmapQ_no_L1_orphans:
   "invs' s \<Longrightarrow> bitmapQ_no_L1_orphans s"
@@ -3064,12 +3643,13 @@ lemma invs'_bitmapQ_no_L1_orphans:
 
 lemma invs_ksCurDomain_maxDomain' [elim!]:
   "invs' s \<Longrightarrow> ksCurDomain s \<le> maxDomain"
-  by (simp add: invs'_def valid_state'_def)
+  by (simp add: invs'_def)
 
+(* FIXME RT: not going to work any more like this:
 lemma simple_st_tcb_at_state_refs_ofD':
   "st_tcb_at' simple' t s \<Longrightarrow> bound_tcb_at' (\<lambda>x. tcb_bound_refs' x = state_refs_of' s t) t s"
   by (fastforce simp: pred_tcb_at'_def obj_at'_def state_refs_of'_def
-                      projectKO_eq project_inject)
+                      projectKO_eq project_inject) *)
 
 lemma cur_tcb_arch' [iff]:
   "cur_tcb' (ksArchState_update f s) = cur_tcb' s"
@@ -3081,28 +3661,22 @@ lemma cur_tcb'_machine_state [simp]:
 
 lemma invs_no_0_obj'[elim!]:
   "invs' s \<Longrightarrow> no_0_obj' s"
-  by (simp add: invs'_def valid_state'_def valid_pspace'_def)
+  by (simp add: invs'_def valid_pspace'_def)
 
 lemma invs'_gsCNodes_update[simp]:
   "invs' (gsCNodes_update f s') = invs' s'"
-  apply (clarsimp simp: invs'_def valid_state'_def valid_queues_def valid_queues_no_bitmap_def
-             bitmapQ_defs
-             valid_queues'_def valid_irq_node'_def valid_irq_handlers'_def
-             irq_issued'_def irqs_masked'_def valid_machine_state'_def
-             cur_tcb'_def)
-  apply (cases "ksSchedulerAction s'")
-  apply (simp_all add: ct_in_state'_def tcb_in_cur_domain'_def ct_idle_or_in_cur_domain'_def ct_not_inQ_def)
+  apply (clarsimp simp: invs'_def valid_queues_def valid_queues_no_bitmap_def bitmapQ_defs
+                        valid_queues'_def valid_release_queue_def valid_release_queue'_def
+                        valid_irq_node'_def valid_irq_handlers'_def irq_issued'_def irqs_masked'_def
+                        valid_machine_state'_def valid_dom_schedule'_def)
   done
 
 lemma invs'_gsUserPages_update[simp]:
   "invs' (gsUserPages_update f s') = invs' s'"
-  apply (clarsimp simp: invs'_def valid_state'_def valid_queues_def valid_queues_no_bitmap_def
-             bitmapQ_defs
-             valid_queues'_def valid_irq_node'_def valid_irq_handlers'_def
-             irq_issued'_def irqs_masked'_def valid_machine_state'_def
-             cur_tcb'_def)
-  apply (cases "ksSchedulerAction s'")
-  apply (simp_all add: ct_in_state'_def ct_idle_or_in_cur_domain'_def tcb_in_cur_domain'_def ct_not_inQ_def)
+  apply (clarsimp simp: invs'_def valid_queues_def valid_queues_no_bitmap_def bitmapQ_defs
+                        valid_queues'_def valid_release_queue_def valid_release_queue'_def
+                        valid_irq_node'_def valid_irq_handlers'_def irq_issued'_def irqs_masked'_def
+                        valid_machine_state'_def valid_dom_schedule'_def)
   done
 
 lemma invs_queues_tcb_in_cur_domain':
@@ -3118,12 +3692,32 @@ lemma pred_tcb'_neq_contra:
   by (clarsimp simp: pred_tcb_at'_def obj_at'_def)
 
 lemma invs'_ksDomSchedule:
-  "invs' s \<Longrightarrow> KernelStateData_H.ksDomSchedule s = KernelStateData_H.ksDomSchedule (newKernelState undefined)"
-unfolding invs'_def valid_state'_def by clarsimp
+  "invs' s \<Longrightarrow> ksDomSchedule s = ksDomSchedule (newKernelState undefined)"
+  unfolding invs'_def valid_dom_schedule'_def by clarsimp
 
 lemma invs'_ksDomScheduleIdx:
-  "invs' s \<Longrightarrow> KernelStateData_H.ksDomScheduleIdx s < length (KernelStateData_H.ksDomSchedule (newKernelState undefined))"
-unfolding invs'_def valid_state'_def by clarsimp
+  "invs' s \<Longrightarrow> ksDomScheduleIdx s < length (ksDomSchedule (newKernelState undefined))"
+  unfolding invs'_def valid_dom_schedule'_def by clarsimp
+
+lemmas invs'_implies =
+  invs_iflive'
+  invs_unsafe_then_cap'
+  invs_no_0_obj'
+  invs_pspace_aligned'
+  invs_pspace_distinct'
+  invs_pspace_bounded'
+  invs_arch_state'
+  invs_valid_global'
+  invs_mdb'
+  invs_valid_objs'
+  invs_valid_objs_size'
+  invs_valid_pspace'
+  invs_queues
+  invs_queues'
+  invs_valid_release_queue
+  invs_valid_release_queue'
+  invs_sym_list_refs_of_replies'
+  invs_valid_replies'
 
 lemma valid_bitmap_valid_bitmapQ_exceptE:
   "\<lbrakk> valid_bitmapQ_except d p s ; (bitmapQ d p s \<longleftrightarrow> ksReadyQueues s (d,p) \<noteq> []) ;
@@ -3246,16 +3840,179 @@ private lemma ko_at_defn_ko_wp_at':
   by (clarsimp simp: ko_at'_defn_def obj_at'_real_def
                      ko_wp_at'_def project_inject)
 
-method normalise_obj_at' =
+(* FIXME: normalise_obj_at' sometimes doesn't normalise obj_at' unless you use it twice.
+          See VER-1364 for more details. *)
+private method normalise_obj_at'_step =
   (clarsimp?, elim obj_at_ko_at'[folded ko_at'_defn_def, elim_format],
    clarsimp simp: ko_at_defn_rewr ko_at_defn_pred_tcb_at' ko_at_defn_ko_wp_at',
    ((drule(1) ko_at_defn_uniqueD)+)?,
    clarsimp simp: ko_at'_defn_def)
 
+method normalise_obj_at' =
+  normalise_obj_at'_step, normalise_obj_at'_step?
+
 end
+
+lemma valid_replies'D:
+  "valid_replies' s \<Longrightarrow> is_reply_linked rptr s
+   \<Longrightarrow> \<exists>tptr. replyTCBs_of s rptr = Some tptr
+              \<and> st_tcb_at' ((=) (BlockedOnReply (Some rptr))) tptr s"
+  apply (clarsimp simp: valid_replies'_def)
+  apply (drule_tac x=rptr in spec)
+  apply fastforce
+  done
+
+lemma valid_replies'_no_tcb:
+  "\<lbrakk>replyTCBs_of s rptr = None; valid_replies' s\<rbrakk>
+   \<Longrightarrow> \<not> is_reply_linked rptr s"
+  by (force simp: valid_replies'_def opt_map_def)
+
+lemma valid_replies'_other_state:
+  "\<lbrakk>replyTCBs_of s rptr = Some tptr;
+    st_tcb_at' P tptr s; \<not> P (BlockedOnReply (Some rptr));
+    valid_replies' s\<rbrakk>
+   \<Longrightarrow> \<not> is_reply_linked rptr s"
+  apply (clarsimp simp: valid_replies'_def)
+  apply (drule_tac x=rptr in spec)
+  apply (fastforce simp: pred_tcb_at'_def obj_at'_def)+
+  done
+
+lemma valid_replies'_sc_asrtD:
+  "valid_replies'_sc_asrt rptr s \<Longrightarrow> replySCs_of s rptr \<noteq> None
+   \<Longrightarrow> (\<exists>tptr. replyTCBs_of s rptr = Some tptr
+               \<and> st_tcb_at' ((=) (BlockedOnReply (Some rptr))) tptr s)"
+  by (clarsimp simp: valid_replies'_sc_asrt_def)
+
+lemma valid_replies'_sc_asrt_replySC_None:
+  "\<lbrakk>valid_replies'_sc_asrt rptr s; replyTCBs_of s rptr = Some tptr;
+    st_tcb_at' P tptr s; \<not> P (BlockedOnReply (Some rptr))\<rbrakk>
+   \<Longrightarrow> replySCs_of s rptr = None"
+  by (force simp: valid_replies'_sc_asrt_def pred_tcb_at'_def obj_at'_def)
+
+lemma valid_replies'_no_tcb_not_linked:
+  "\<lbrakk>replyTCBs_of s replyPtr = None;
+    valid_replies' s; valid_replies'_sc_asrt replyPtr s\<rbrakk>
+    \<Longrightarrow> \<not> is_reply_linked replyPtr s \<and> replySCs_of s replyPtr = None"
+  apply (clarsimp simp: valid_replies'_def valid_replies'_sc_asrt_def)
+  apply (drule_tac x=replyPtr in spec)
+  apply clarsimp
+  done
+
+lemma valid_replies'_sc_asrt_lift:
+  assumes x: "\<And>P. f \<lbrace>\<lambda>s. P (replySCs_of s)\<rbrace>"
+  assumes y: "\<And>P. f \<lbrace>\<lambda>s. P (replyTCBs_of s)\<rbrace>"
+  assumes z: "\<And>rptr t. f \<lbrace>st_tcb_at' ((=) (BlockedOnReply rptr)) t\<rbrace>"
+  shows "f \<lbrace>valid_replies'_sc_asrt replyPtr\<rbrace>"
+  unfolding valid_replies'_sc_asrt_def
+  by (wpsimp wp: hoare_vcg_imp_lift' x y z hoare_vcg_ex_lift)
+
+lemma valid_replies'_lift:
+  assumes rNext: "\<And>P. f \<lbrace>\<lambda>s. P (replyNexts_of s)\<rbrace>"
+  and rPrev: "\<And>P. f \<lbrace>\<lambda>s. P (replyPrevs_of s)\<rbrace>"
+  and rTCB: "\<And>P. f \<lbrace>\<lambda>s. P (replyTCBs_of s)\<rbrace>"
+  and st: "\<And>rptr p. f \<lbrace>st_tcb_at' ((=) (BlockedOnReply rptr)) p\<rbrace>"
+  shows "\<lbrace>valid_replies'\<rbrace> f \<lbrace>\<lambda>_. valid_replies'\<rbrace>"
+  unfolding valid_replies'_def
+  by (wpsimp wp: hoare_vcg_imp_lift' rNext rPrev rTCB st hoare_vcg_all_lift hoare_vcg_ex_lift)
+
+lemma cteCaps_of_ctes_of_lift:
+  "(\<And>P. f \<lbrace>\<lambda>s. P (ctes_of s)\<rbrace>) \<Longrightarrow> f \<lbrace>\<lambda>s. P (cteCaps_of s)\<rbrace>"
+  unfolding cteCaps_of_def .
+
+lemmas ctes_of_cteCaps_of_lift = cteCaps_of_ctes_of_lift
 
 add_upd_simps "invs' (gsUntypedZeroRanges_update f s)"
   (obj_at'_real_def)
 declare upd_simps[simp]
+
+(* sym_heap *)
+
+lemma sym_refs_replyNext_replyPrev_sym:
+  "sym_refs (list_refs_of_replies' s') \<Longrightarrow>
+    replyNexts_of s' rp = Some rp' \<longleftrightarrow> replyPrevs_of s' rp' = Some rp"
+  apply (rule iffI; clarsimp simp: projectKO_opts_defs split: kernel_object.split_asm)
+   apply (drule_tac tp=ReplyNext and y=rp' and x=rp in sym_refsD[rotated])
+    apply (clarsimp simp: map_set_def opt_map_red list_refs_of_reply'_def projectKO_opt_reply)
+   apply (clarsimp simp: opt_map_red map_set_def get_refs_def2 list_refs_of_reply'_def
+                  split: option.split_asm)
+  apply (drule_tac tp=ReplyPrev and y=rp and x=rp' in sym_refsD[rotated])
+   apply (clarsimp simp: map_set_def opt_map_red list_refs_of_reply'_def projectKO_opt_reply)
+  by (clarsimp simp: opt_map_red map_set_def get_refs_def2 list_refs_of_reply'_def
+              split: option.split_asm)
+
+lemma reply_sym_heap_Next_Prev:
+  "sym_refs (list_refs_of_replies' s') \<Longrightarrow> sym_heap (replyNexts_of s') (replyPrevs_of s')"
+  using sym_refs_replyNext_replyPrev_sym by (clarsimp simp: sym_heap_def)
+
+lemmas reply_sym_heap_Prev_Next
+  = sym_heap_symmetric[THEN iffD1, OF reply_sym_heap_Next_Prev]
+
+lemmas sym_refs_replyNext_None
+  = sym_heap_None[OF reply_sym_heap_Next_Prev]
+
+lemmas sym_refs_replyPrev_None
+  = sym_heap_None[OF reply_sym_heap_Prev_Next]
+
+lemmas sym_refs_reply_heap_path_doubly_linked_Prevs_rev
+  = sym_heap_path_reverse[OF reply_sym_heap_Next_Prev]
+
+lemmas sym_refs_reply_heap_path_doubly_linked_Nexts_rev
+  = sym_heap_path_reverse[OF reply_sym_heap_Prev_Next]
+
+lemmas sym_refs_replyNext_heap_ls_Cons
+  = sym_heap_ls_rev_Cons[OF reply_sym_heap_Next_Prev]
+
+lemmas sym_refs_replyPrev_heap_ls_Cons
+  = sym_heap_ls_rev_Cons[OF reply_sym_heap_Prev_Next]
+
+lemmas sym_refs_replyNext_heap_ls
+  = sym_heap_ls_rev[OF reply_sym_heap_Next_Prev]
+
+lemmas sym_refs_replyPrev_heap_ls
+  = sym_heap_ls_rev[OF reply_sym_heap_Prev_Next]
+
+(* end: sym_heap *)
+
+lemma no_replySC_valid_replies'_sc_asrt:
+  "replySCs_of s r = None \<Longrightarrow> valid_replies'_sc_asrt r s"
+  unfolding valid_replies'_sc_asrt_def
+  by (simp)
+
+(** sc_with_reply' **)
+
+definition sc_with_reply' :: "obj_ref \<Rightarrow> kernel_state \<Rightarrow> obj_ref option" where
+  "sc_with_reply' rp s'
+     \<equiv> the_pred_option (\<lambda>sc_ptr. \<exists>xs. heap_ls (replyPrevs_of s') (scReplies_of s' sc_ptr) xs
+                                       \<and> rp \<in> set xs)"
+
+lemma sc_with_reply'_SomeD:
+  "sc_with_reply' rp s' = Some scp \<Longrightarrow>
+     \<exists>xs. heap_ls (replyPrevs_of s') (scReplies_of s' scp) xs
+                     \<and> rp \<in> set xs"
+  by (clarsimp simp: sc_with_reply'_def dest!: the_pred_option_SomeD)
+
+lemma sc_with_reply'_NoneD:
+  "sc_with_reply' rp s' = None \<Longrightarrow>
+     \<nexists>!scp. \<exists>xs. heap_ls (replyPrevs_of s') (scReplies_of s' scp) xs
+                     \<and> rp \<in> set xs"
+  by (clarsimp simp: sc_with_reply'_def the_pred_option_def split: if_split_asm)
+
+definition "updateTimeStamp_independent (P :: kernel_state \<Rightarrow> bool)
+  \<equiv> \<forall>f g s. P s \<longrightarrow> P (s\<lparr>ksCurTime := f (ksCurTime s), ksConsumedTime := g (ksConsumedTime s)\<rparr>)"
+
+lemma updateTimeStamp_independentI[intro!, simp]:
+  "\<lbrakk>\<And>s f g. P (s\<lparr>ksCurTime := f (ksCurTime s), ksConsumedTime := g (ksConsumedTime s)\<rparr>) = P s\<rbrakk>
+   \<Longrightarrow> updateTimeStamp_independent P"
+  by (simp add: updateTimeStamp_independent_def)
+
+definition "domain_time_independent_H (P :: kernel_state \<Rightarrow> bool)
+  \<equiv> \<forall>f s. P s \<longrightarrow>
+           P (s\<lparr>ksDomainTime := f (ksDomainTime s)\<rparr>)"
+
+lemma domain_time_independent_HI[intro!, simp]:
+   "\<lbrakk>\<And>s f. P (s\<lparr>ksDomainTime := f (ksDomainTime s)\<rparr>)
+            = P s\<rbrakk>
+    \<Longrightarrow> domain_time_independent_H P"
+  by (simp add: domain_time_independent_H_def)
 
 end
