proof/refine/RISCV64/Machine_R.thy
@@ -12,15 +12,41 @@ theory Machine_R
 imports Bits_R
 begin
 
-definition "irq_state_independent_H (P :: kernel_state \<Rightarrow> bool)\<equiv>
-              \<forall>(f :: nat \<Rightarrow> nat) (s :: kernel_state). P s \<longrightarrow> P (s\<lparr>ksMachineState := ksMachineState s
-                                \<lparr>irq_state := f (irq_state (ksMachineState s))\<rparr>\<rparr>)"
+definition irq_state_independent_H :: "(kernel_state \<Rightarrow> bool) \<Rightarrow> bool" where
+  "irq_state_independent_H P
+    \<equiv> \<forall>f s. P s \<longrightarrow> P (s\<lparr>ksMachineState := ksMachineState s \<lparr>irq_state := f (irq_state (ksMachineState s))\<rparr>\<rparr>)"
 
 lemma irq_state_independent_HI[intro!, simp]:
   "\<lbrakk>\<And>s f. P (s\<lparr>ksMachineState := ksMachineState s
               \<lparr>irq_state := f (irq_state (ksMachineState s))\<rparr>\<rparr>) = P s\<rbrakk>
    \<Longrightarrow> irq_state_independent_H P"
   by (simp add: irq_state_independent_H_def)
+
+definition  getCurrentTime_independent_H :: "(kernel_state \<Rightarrow> bool) \<Rightarrow> bool" where
+  "getCurrentTime_independent_H P
+    \<equiv> \<forall>f s. P s \<longrightarrow>
+             P (s\<lparr>ksMachineState :=
+                       ksMachineState s\<lparr>last_machine_time :=
+                          f (last_machine_time (ksMachineState s)) (time_state (ksMachineState s))\<rparr>\<rparr>)"
+
+lemma getCurrentTime_independent_HI[intro!, simp]:
+   "\<lbrakk>\<And>s f. P (s\<lparr>ksMachineState
+              := (ksMachineState s)\<lparr>last_machine_time :=
+                                f (last_machine_time (ksMachineState s)) (time_state (ksMachineState s))\<rparr>\<rparr>)
+           = P s\<rbrakk>
+    \<Longrightarrow> getCurrentTime_independent_H P"
+   by (simp add: getCurrentTime_independent_H_def)
+
+definition  time_state_independent_H :: "(global.kernel_state \<Rightarrow> bool) \<Rightarrow> bool" where
+  "time_state_independent_H P
+    \<equiv> \<forall>f s. P s \<longrightarrow>
+             P (s\<lparr>ksMachineState := ksMachineState s\<lparr>time_state := f (time_state (ksMachineState s))\<rparr>\<rparr>)"
+
+lemma time_state_independent_HI[intro!, simp]:
+   "\<lbrakk>\<And>s f. P (s\<lparr>ksMachineState := ksMachineState s\<lparr>time_state := f (time_state (ksMachineState s))\<rparr>\<rparr>)
+            = P s\<rbrakk>
+    \<Longrightarrow> time_state_independent_H P"
+   by (simp add: time_state_independent_H_def)
 
 context begin interpretation Arch . (*FIXME: arch_split*)
 
@@ -54,7 +80,7 @@ lemma dmo_maskInterrupt:
 lemma dmo_maskInterrupt_True:
   "\<lbrace>invs'\<rbrace> doMachineOp (maskInterrupt True irq) \<lbrace>\<lambda>_. invs'\<rbrace>"
   apply (wp dmo_maskInterrupt)
-  apply (clarsimp simp: invs'_def valid_state'_def)
+  apply (clarsimp simp: invs'_def valid_dom_schedule'_def)
   apply (simp add: valid_irq_masks'_def valid_machine_state'_def
                    ct_not_inQ_def ct_idle_or_in_cur_domain'_def tcb_in_cur_domain'_def)
   done
