proof/refine/RISCV64/ArchMove_R.thy
@@ -24,8 +24,8 @@ context begin interpretation Arch .
 definition ppn_len :: nat where
   "ppn_len \<equiv> LENGTH(pte_ppn_len)"
 
-(* Move to Deterministic_AI *)
-crunch valid_etcbs[wp]: copy_global_mappings valid_etcbs (wp: mapM_x_wp')
+\<comment> \<open>(* Move to Deterministic_AI *)
+crunch valid_etcbs[wp]: copy_global_mappings valid_etcbs (wp: mapM_x_wp' crunch_wps)\<close>
 
 lemma get_pt_mapM_x_lower:
   assumes g: "\<And>P pt x. \<lbrace> \<lambda>s. P (kheap s pt_ptr) \<rbrace> g pt x \<lbrace> \<lambda>_ s. P (kheap s pt_ptr) \<rbrace>"
